division on sevral files, some proofs are added Key Functor added

Json.v
@@ -3,70 +3,46 @@ Require Import Lists.List.
 Require Import Coq.Init.Nat.
 Require Import Coq.Program.Basics.
 
+Require Export KeyMaps. 
+Require Export CommonHelpers.
+Require Export StringHelpers.
+
 Import ListNotations.
 
 Local Open Scope list_scope.
 Local Open Scope string_scope.
 
-Definition natToDigit (n : nat) : string :=
-  match n with
-    | 0 => "0"
-    | 1 => "1"
-    | 2 => "2"
-    | 3 => "3"
-    | 4 => "4"
-    | 5 => "5"
-    | 6 => "6"
-    | 7 => "7"
-    | 8 => "8"
-    | _ => "9"
-  end.
-
-Fixpoint writeNatAux (time n : nat) (acc : string) : string :=
-  let acc' := (natToDigit (n mod 10)) ++ acc in
-  match time with
-    | 0 => acc'
-    | S time' =>
-      match n / 10 with
-        | 0 => acc'
-        | n' => writeNatAux time' n' acc'
-      end
-  end.
-
-Definition writeNat (n : nat) : string :=
-  writeNatAux n n "".
-
-Example writeNat174: writeNat 174 = "174".
-Proof.
- auto.
-Qed. 
-
-Example writeNat10: writeNat 10 = "10".
-Proof.
- auto.
-Qed. 
-
-Example writeNat0: writeNat 0 = "0".
-Proof.
- auto.
-Qed. 
-
+Module StringKeySig <: KeyMaps.KeySig.
 Definition key := string.
-Definition data := string.
+Definition eqKey := fun s1 s2 => if (string_dec s1 s2) then true else false.
+Lemma eqKey_refl: forall s1 s2, eqKey s1 s2 = true <-> s1 = s2.
+Proof.
+ intros. split. unfold eqKey.
+ remember (string_dec s1 s2). destruct s.
+ auto. discriminate.
+ intros. unfold eqKey. remember (string_dec s1 s2). destruct s.
+ auto. unfold not in n. clear Heqs. apply n in H.
+ inversion H.
+Defined. 
+End StringKeySig.
 
-Inductive key_map {X} := 
-| empty: key_map
-| mapkv: key -> X -> key_map -> key_map.
+Module StringKeyMap := KeyMaps.KeyMap StringKeySig.
+Export StringKeySig.
+Export StringKeyMap.
 
-Inductive json :=
-| json_data: data -> json
+
+(*transform this to module sig or variable*)
+Definition JsonData := string.
+
+Inductive json : Set :=
+| json_data: JsonData -> json
 | json_list : list json  -> json
 | json_map: @key_map json -> json.
 
 Module JsonNotations.
 Notation "{ }" := (json_map empty): json_scope.
 Infix "#" := mapkv (at level 0): json_scope.
-Notation "{ k # v }" := (json_map (mapkv k v empty))
+Notation "{ k # v }" := (json_map (mapkv k v empty key json))
                                  (right associativity): json_scope.
 Notation "{ kv1 , .. , kv2 }" := (json_map (kv1 .. (kv2 empty) ..))
                                  (right associativity): json_scope.
@@ -82,63 +58,7 @@ Import JsonNotations.
 Local Open Scope json_scope.
 Delimit Scope json_scope with json.
 
-Check ($"foo").
-Check { "foo" # $"bar" }.
-Check ('([$"foo"]%list)).
-Check {"1" # $"Andy" , "2" # $"Peter"}.
 
-Fixpoint firstSome {X} (l: list (option X)): option X :=
-match l with
-| [] => None
-| (Some x):: _ => Some x
-| None :: l => firstSome l
-end.
-
-Fixpoint firstSome_ind' {X} (n:nat) (l: list (option X)): option (nat*X) :=
-match l with
-| [] => None
-| (Some x):: _ => Some (n, x)
-| None :: l => firstSome_ind' (S n) l
-end.
-
-Definition firstSome_ind {X} := @firstSome_ind' X 0.
-
-Fixpoint mapmap {X Y} (f: X -> Y) (m: @key_map X) :=
-match m with
-| empty => empty
-| mapkv k v kvs => mapkv k (f v) (mapmap f kvs)
-end. 
-
-Fixpoint mapkeymap {X Y} (f: key -> X -> Y) (m: @key_map X) : list Y :=
-match m with
-| empty => []
-| mapkv k v kvs => (f k v) :: (mapkeymap f kvs)
-end.
-
-Fixpoint mapkeymap' {X Y} (f: X -> Y) (m: @key_map X) : list Y :=
-match m with
-| empty => []
-| mapkv k v kvs => (f v) :: (mapkeymap' f kvs)
-end. 
-
-Definition mapkeymap'' {X Y} (f: X -> Y) (m: @key_map X) : list Y:=
-mapkeymap (fun _ v => f v) m.
-
-Lemma mapkeymap''equal: forall X Y (f: X -> Y) m,
-                 mapkeymap'' f m = mapkeymap' f m.
-Proof.
- intros. unfold mapkeymap''.
- induction m. simpl. auto.
- simpl. rewrite IHm. auto.
-Qed.
-
-Fixpoint merge_maps {X} (m1 m2: @key_map X) :=
-match m1 with
-| empty => m2
-| mapkv k v m1' => merge_maps m1' (mapkv k v m2)
-end.
-
-Definition valuelist {X} := mapkeymap' (@id X).
 
 Definition jsonmap (f: json -> json) (j: json) :=
 match j with
@@ -147,13 +67,8 @@ match j with
 | & m => & (mapmap f m)
 end.
 
-Eval compute in (jsonmap (fun x => {}) {"foo" # $"foo", "bar" # $"bar"}).
-
-Definition mlookup {X} (m: @key_map X) (k: key) :=
-firstSome (mapkeymap (fun k' v => if (string_dec k k') then Some v else None) m).
-
-Definition jpoint:Set := key + nat.
-Definition jpath  := list jpoint.
+Definition jpoint: Set := key + nat.
+Definition jpath:= list jpoint.
 
 Fixpoint json_get (kk: jpoint) (j: json) {struct j}: option json :=
 match kk with
@@ -167,17 +82,6 @@ match kk with
            end
 end.
 
-Eval compute in (json_get (inl "foo") {"foo" # $"Andy", "bar" #  $"Peter"}).
-Eval compute in (json_get (inl "bar") {"foo" # $"Andy", "bar" #  $"Peter"}).
-Eval compute in (json_get (inl "baz") {"foo" # $"Andy", "bar" #  $"Peter"}).
-
-Eval compute in (json_get (inr 0) '[$"Andy"; $"Peter"]).
-Eval compute in (json_get (inr 1) '[$"Andy"; $"Peter"]).
-Eval compute in (json_get (inr 2) '[$"Andy"; $"Peter"]).
-
-Eval compute in (json_get (inr 0) $"Andy").
-Eval compute in (json_get (inl "foo") $"Andy").
-
 Fixpoint json_getin (lk: jpath) (j: json): option json :=
 match lk with
 | [] => Some j
@@ -188,521 +92,11 @@ match lk with
            end 
 end.
 
-Eval compute in (json_getin [inl "foo"; inr 1] 
-                 {"foo" # '[$"Andy"; $"Peter"]}).
-
-Fixpoint flatten {X} (ll: list (list X)) : list X :=
-match ll with
-| [] => []
-| l::ls => app l (flatten ls)
-end.
-
-Fixpoint map2list (m: key_map) : list json :=
+Fixpoint keymap_list (m: key_map) : list json :=
 match m with
 | empty => []
-| mapkv k v kvs => v::(map2list kvs)
+| mapkv k v kvs => v::(keymap_list kvs)
 end.
-
-Inductive tree (X Y: Type) : Type :=
-| tleaf : X -> @tree X Y
-| tlbranch : list (nat*tree X Y) -> tree X Y
-| tmbranch : list (Y*tree X Y) -> tree X Y.
-
-(*the empty tree can be written as "tlbranch []"*)
-
-Arguments tleaf [X] [Y].
-Arguments tlbranch [X] [Y].
-Arguments tmbranch [X] [Y].
-
-Definition jtree := tree data key.
-
-Fixpoint indexate_with' {X Y} (n:nat) (f: nat -> Y) (l: list X) :=
-match l with
-| [] => []
-| x::xs => (f n,x)::(indexate_with' (S n) f xs)
-end.
-
-Definition indexate {X} := @indexate_with' X nat 0 (@id nat).
-Definition indexate_with {X Y} := @indexate_with' X Y 0.
-
-Fixpoint json_tree (j: json): jtree :=
-match j with
-| $s => tleaf s
-| 'l => tlbranch (indexate (map json_tree l))
-| &m => let fix map_tree (mm: @key_map json) :=
-            match mm with
-            | empty => []
-            | mapkv k v kvs => (k, json_tree v)::map_tree kvs 
-            end in
-        tmbranch (map_tree m)
-end.
-
-
-Eval compute in (json_tree 
-                 ('[{"foo" # '[$"Andy"; $"Peter"]}; 
-                    {"bar" # $"Good"};
-                    {"baz" # {"x" # '[$"d"; $"f"]}}])).
-
-Fixpoint tree_json (jt: jtree): option json :=
-match jt with
-| tleaf s => Some $s
-| tlbranch lt => let l := fold_right (fun (kt:nat*jtree) l =>
-                                    match l with
-                                    | Some l => let mj := tree_json (snd kt) in
-                                                       match mj with
-                                                       | Some j => Some (cons j l)
-                                                       | None => None
-                                                       end
-                                    | _ => None
-                                    end) (Some []) lt in
-                           match l with
-                           | None => None
-                           | Some l => Some 'l
-                           end
-| tmbranch mt => let m := fold_right (fun (kt: key*jtree) m =>  
-                                        let (k, t) := kt in
-                                        match k, m with 
-                                        | k, Some m => let mj := tree_json t in
-                                                           match mj with
-                                                           | Some j => Some (mapkv k j m)
-                                                           | None => None
-                                                           end
-                                        | _, _ => None 
-                                        end) (Some empty) mt in
-                                  match m with
-                                  | None => None
-                                  | Some m => Some &m
-                                  end
-end.
-
-
-Eval compute in (tree_json (json_tree 
-                 ('[{"foo" # '[$"Andy"; $"Peter"]}; 
-                    {"bar" # $"Good"};
-                    {"baz" # {"x" # '[$"d"; $"f"]}}]))).
-
-Example eqtree1 : (tree_json (json_tree 
-                 ('[{"foo" # '[$"Andy"; $"Peter"]}; 
-                    {"bar" # $"Good"};
-                    {"baz" # {"x" # '[$"d"; $"f"]}}]))) =
-                    Some '[{"foo" # '[$"Andy"; $"Peter"]}; 
-                    {"bar" # $"Good"};
-                    {"baz" # {"x" # '[$"d"; $"f"]}}].
-Proof.
- auto.
-Qed.
-
-Inductive MergeStrategyIn := SMergeRight | SReplace | SMergeLeft | SExchange. 
-Inductive MergeStrategyOut := SRemoveOrigin | SLeaveOrigin.
-Inductive NameStrategy := 
-| SRenameNode: key -> NameStrategy
-| SLeaveNodeName: NameStrategy.
-
-Inductive MergeStrategyT := 
-| MergeStrategy: MergeStrategyIn -> MergeStrategyOut ->
-                 NameStrategy -> NameStrategy -> MergeStrategyT.
-
-Definition MergeStrategy0 := MergeStrategy SMergeRight SLeaveOrigin 
-                             SLeaveNodeName SLeaveNodeName.
-
-Definition indexNat (n: nat):  string :=
-"#" ++ (writeNat n).
-
-Definition merge_trees (t1 t2: jtree) (s: MergeStrategyT) : jtree :=
-match t1,t2 with
-| tleaf s1, tleaf s2 => tlbranch (indexate [t1; t2])
-
-| tleaf s1, tlbranch tl2 => tlbranch (indexate (t1::(map snd tl2)))
-| tlbranch tl1, tleaf s2 => tlbranch (indexate (app (map snd tl1) [t2]))
-| tlbranch tl1, tlbranch tl2 => tlbranch (indexate (app (map snd tl1) (map snd tl2)))
-
-| tleaf s1, tmbranch tm2 => tmbranch ((indexNat 0, t1)::tm2)
-| tmbranch tm1, tleaf s2 =>  tmbranch (app tm1 [(indexNat 0, t2)])
-| tmbranch tm1, tmbranch tm2 => tmbranch (app tm1 tm2)
-
-| tlbranch tl1, tmbranch tm2 => tmbranch (app (indexate_with indexNat (map snd tl1)) tm2)
-| tmbranch tm1, tlbranch tl2 => tmbranch (app tm1 (indexate_with indexNat (map snd tl2)))
-end.
-
-
-
-Definition tlookup {X} (tm: list (key*(tree X key))) (k: key) :=
-firstSome (map (fun (k'v: key*(tree X key)) => let (k', v) := k'v in
-                           if (string_dec k k') then Some v else None) tm).
-
-Definition tlookup_ind {X} (tm: list (key*(tree X key))) (k: key) :=
-firstSome_ind (map (fun (k'v: key*(tree X key)) => let (k', v) := k'v in
-                           if (string_dec k k') then Some v else None) tm).
-
-
-Fixpoint tree_get (kk: jpoint) (jt: jtree) {struct jt}: option (nat*jtree) :=
-match kk with
-| inl k => match jt with
-              | tmbranch tm => tlookup_ind tm k
-              | _ => None
-           end
-| inr k => match jt with
-              | tlbranch tl  => nth_error tl k
-              | _ => None
-           end
-end.
-
-Fixpoint tree_getin (lk: jpath) (jt: jtree): option jtree :=
-match lk with
-| [] => Some jt
-| k::ks => let mjt' := tree_get k jt in
-           match mjt' with
-           | None => None
-           | Some (_,jt') => tree_getin ks jt'
-           end 
-end.
-
-Fixpoint replace {X} (n: nat) (l: list X) (x: X) :=
-match n,l with
-| _, [] => []
-| 0, (a::l') => x::l'
-| S n', (a::l') => a::(replace n' l' x)
-end.
-
-Eval compute in (replace 0 [1;2] 0).
-Eval compute in (replace 1 [1;2] 0).
-Eval compute in (replace 2 [1;2] 0).
-Eval compute in (replace 0 [] 0).
-Eval compute in (replace 0 [1] 0).
-
-
-Fixpoint tree_setin (lk: jpath) (to_jt jt: jtree): jtree :=
-match lk with
-| [] => jt
-| k::ks => let mjt' := tree_get k to_jt in
-           match mjt' with
-           | None => to_jt
-           | Some (n, to_jt') => let nt := tree_setin ks to_jt' jt in
-                                 match k, to_jt with
-                                 | inr k, tlbranch tl => (tlbranch (replace n tl (k, nt)))
-                                 | inl k, tmbranch tm => (tmbranch (replace n tm (k, nt)))
-                                 | _,_ => to_jt
-                                 end
-           end 
-end.
-
-Definition tree_modify (lk_in: jpath) (jt: jtree) (f: jtree -> jtree) : jtree :=
-let mjt' := tree_getin lk_in jt in
-match mjt' with
-| Some jt' => tree_setin lk_in jt (f jt')
-| None => jt
-end.
-
-Example tsetin1 : tree_json 
-                  (tree_setin [inr 2; inl "baz"; inl "x"; inr 1]
-                   (json_tree '[{"foo" # '[$"Andy"; $"Peter"]}; 
-                     {"bar" # $"Good"};
-                     {"baz" # {"x" # '[$"d"; $"f"]}}]) (tleaf "e")) = 
-                  Some '[{"foo" # '[$"Andy"; $"Peter"]}; 
-                    {"bar" # $"Good"};
-                    {"baz" # {"x" # '[$"d"; $"e"]}}].
-Proof. auto. Qed.
-
-Definition concat_tree_with (d: data) (jt: jtree): jtree :=
-match jt with
-| tleaf s => tleaf s
-| tlbranch tl => tleaf (fold_right (fun i r => match i with
-                                        | (_, tleaf s) => if (string_dec r "") then s 
-                                                          else (s ++ d ++ r)
-                                        | _ => r
-                                        end) ""  tl)
-| tmbranch tm => tleaf (fold_right (fun i r => match i with
-                                        | (_, tleaf s) => if (string_dec r "") then s 
-                                                          else (s ++ d ++ r)
-                                        | _ => r
-                                        end) ""  tm)
-end.
-
-Check split.
-
-
-Example tmodify1: tree_json (tree_modify [inr 0; inl "foo"]
-                  (json_tree ('[{"foo" # '[$"Andy"; $"Peter"]}; 
-                    {"bar" # $"Good"};
-                    {"baz" # {"x" # '[$"d"; $"f"]}}])) (concat_tree_with " ")) = 
-                  Some '[{"foo" # $"Andy Peter"}; 
-                    {"bar" # $"Good"};
-                    {"baz" # {"x" # '[$"d"; $"f"]}}].
-Proof. auto. Qed.
-
-Example tsetin2: tree_json (tree_setin [inr 2; inl "baz"; inl "x"; inr 0]
-                 (json_tree ('[{"foo" # '[$"Andy"; $"Peter"]}; 
-                    {"bar" # $"Good"};
-                    {"baz" # {"x" # '[$"d"; $"f"]}}])) (tleaf "e")) =
-                 Some '[{"foo" # '[$"Andy"; $"Peter"]}; 
-                    {"bar" # $"Good"};
-                    {"baz" # {"x" # '[$"e"; $"f"]}}].
-Proof. auto. Qed.
-
-Definition tree_mergein (lk: jpath) (to_jt jt: jtree) s: jtree :=
-let mjt':= tree_getin lk to_jt in
-match mjt' with
-| None => to_jt
-| Some to_jt' => tree_setin lk to_jt (merge_trees to_jt' jt s)
-end.
-
-Example tmergein1: tree_json (tree_mergein [inr 2; inl "baz"; inl "x"]
-                 (json_tree ('[{"foo" # '[$"Andy"; $"Peter"]}; 
-                    {"bar" # $"Good"};
-                    {"baz" # {"x" # '[$"d"; $"f"]}}])) (tleaf "j") MergeStrategy0) =
-                    Some '[{"foo" # '[$"Andy"; $"Peter"]}; 
-                    {"bar" # $"Good"};
-                    {"baz" # {"x" # '[$"d"; $"f"; $"j"]}}].
-Proof. auto. Qed.
-
-Definition tree_submerge_with (lk_to lk_from: jpath) 
-                              (f: jpath -> jtree -> jtree) (jt: jtree) (s: MergeStrategyT): jtree :=
-let mjt_from' := tree_getin lk_from jt in
-match mjt_from' with
-| Some jt_from' => tree_mergein lk_to jt (f lk_from jt_from') s
-| None => jt
-end.
-
-Definition tree_submerge (lk_to lk_from: jpath) 
-                         (jt: jtree) (s: MergeStrategyT): jtree :=
-tree_submerge_with lk_to lk_from (fun _ jt => jt) jt s.
-
-Example tsmerge1: tree_json (tree_submerge [inr 0] [inr 2; inl "baz"; inl "x"]
-                  (json_tree ('[{"foo" # '[$"Andy"; $"Peter"]}; 
-                    {"bar" # $"Good"};
-                    {"baz" # {"x" # '[$"d"; $"f"]}}])) MergeStrategy0) = 
-                   Some '[{"foo" # '[$"Andy"; $"Peter"], "#0" # $"d", "#1" # $"f"}; 
-                    {"bar" # $"Good"};
-                    {"baz" # {"x" # '[$"d"; $"f"]}}].
-Proof. compute. auto. Qed.
-
-Inductive jnode := 
-| data_node: data -> jnode
-| root_node: jnode.
-
-Definition jtable_row := list jnode.
-
-Fixpoint json_nodes (j: json): jtable_row :=
-match j with
-| $s => [data_node s]
-| 'l => root_node::flatten (map json_nodes l)
-| &m => let fix map_nodes (mm: @key_map json): jtable_row :=
-            match mm with
-            | empty => []
-            | mapkv k v kvs => app (json_nodes v) (map_nodes kvs)
-            end in
-        root_node::map_nodes m
-end.
-
-Fixpoint jtree_nodes (jt: jtree): jtable_row :=
-match jt with
-| tleaf s => [data_node s]
-| tlbranch tl => root_node::flatten (map (compose jtree_nodes snd) tl)
-| tmbranch tm => root_node::flatten (map (compose jtree_nodes snd) tm)
-end.
-
-Eval compute in (json_nodes 
-                 ('[{"foo" # '[$"Andy"; $"Peter"]}; 
-                    {"bar" # $"Good"};
-                    {"baz" # {"x" # '[$"d"; $"f"]}}])).
-
-Eval compute in (jtree_nodes (json_tree
-                 ('[{"foo" # '[$"Andy"; $"Peter"]}; 
-                    {"bar" # $"Good"};
-                    {"baz" # {"x" # '[$"d"; $"f"]}}]))).
-
-Example jtree_json_nodes1: (json_nodes 
-                 ('[{"foo" # '[$"Andy"; $"Peter"]}; 
-                    {"bar" # $"Good"};
-                    {"baz" # {"x" # '[$"d"; $"f"]}}]))=
-                    (jtree_nodes (json_tree
-                 ('[{"foo" # '[$"Andy"; $"Peter"]}; 
-                    {"bar" # $"Good"};
-                    {"baz" # {"x" # '[$"d"; $"f"]}}]))).
-Proof. auto. Qed.
-
-Definition jtable := list (list (option jpoint)). 
-
-Fixpoint list_fill {X} (n: nat) (x:X): list X :=
-match n with
-| O => []
-| S n' => x::(list_fill n' x)
-end.
-
-Definition jtable_fill (n: nat) (a: option jpoint): jtable:=
-list_fill n (list_fill n None).
-
-Definition jtable_set (jt: jtable) (m n: nat) (a: option jpoint) : jtable :=
-let ml := nth_error jt m in
-match ml with
-| Some l => replace m jt (replace n l a)
-| None => jt
-end.
-
-Inductive indjnode := 
-| ind_data_node: nat -> data -> indjnode
-| ind_root_node: nat -> nat -> indjnode.
-
-Fixpoint jtree_table' (m n: nat) (k: option jpoint) (jr: list indjnode)
-                      (jt: jtree) (jtb: jtable) {struct jt}: nat*(list indjnode)*jtable :=
-match jt with
-| tleaf s => let newtb := jtable_set jtb m n k in
-             (S n, app jr [ind_data_node n s] , newtb)
-| tlbranch tl => let newtb':= jtable_set jtb m n k in
-                 let jr' := app jr [ind_root_node m n] in
-                 let fix iter_tree m n k tl jr jtb {struct tl}:=
-                 match tl with
-                 | [] => (n, jr, jtb)
-                 | (a,t)::ts => let (jn'', newtb'') := 
-                                       jtree_table' m n (Some (inr a)) jr t jtb in
-                                let (n', jr'') := jn'' in 
-                                iter_tree m n' None ts jr'' newtb''
-                 end in
-                 iter_tree n (S n) k tl jr' newtb'
-| tmbranch tm => let newtb':= jtable_set jtb m n k in
-                 let jr' := app jr [ind_root_node m n] in
-                 let fix iter_tree m n k tm jr jtb {struct tm}:=
-                 match tm with
-                 | [] => (n, jr, jtb)
-                 | (a,t)::ts => let (jn'', newtb'') := 
-                                       jtree_table' m n (Some (inl a)) jr t jtb in
-                                let (n', jr'') := jn'' in
-                                iter_tree m n' None ts jr'' newtb''
-                 end in
-                 iter_tree n (S n) k tm jr' newtb'
-end.
-
-Definition jtree_table jt := let tb3 := jtree_table' 0 0 None [] jt 
-                             (jtable_fill (length (jtree_nodes jt)) None) in
-                             (snd (fst tb3), snd tb3).
-
-Let j1 := '[{"foo" # '[$"Andy"; $"Peter"]}; 
-                    {"bar" # $"Good"};
-                    {"baz" # {"x" # '[$"d"; $"f"]}}].
-Let t1 := json_tree j1.
-Eval compute in t1.
-Let tn1 := jtree_nodes t1.
-Eval compute in tn1.
-Let jtb10 := jtable_fill (length tn1) None.
-Eval compute in jtb10.
-Let jtb1 := jtree_table t1.
-Eval compute in (jtb1, tn1).
-
-Fixpoint jtable_tree' (n: nat) (m: nat) 
-                      (jr: jtable_row) (jtb: jtable) {struct n}: option jtree :=
-match n with
-| O => None
-| S n' => 
-let mr := nth_error jtb m in
-match mr with
-| Some r => let r' := indexate r in 
-            let fix iter_row r jt :=
-            match r with
-            | [] => jt
-            | (_, None)::rs => iter_row rs jt
-            | (n, Some (inr k))::rs => 
-                                   let md := nth_error jr n in
-                                   iter_row rs match md with
-                                   | Some (data_node s) => 
-                                               match jt with
-                                               | None => Some (tlbranch [(k, tleaf s)])
-                                               | Some (tlbranch tl) => Some (tlbranch (app tl [(k, tleaf s)]))
-                                               | _ => jt
-                                               end
-                                   | Some root_node => let mt' := jtable_tree' n' n jr jtb in
-                                               match mt' with
-                                               | None => jt
-                                               | Some t' => 
-                                                 match jt with
-                                                 | None => Some (tlbranch [(k, t')])
-                                                 | Some (tlbranch tl) => Some (tlbranch (app tl [(k, t')]))
-                                                 | _ => jt
-                                                 end
-                                               end
-                                   | None => None
-                                   end
-            | (n, Some (inl k))::rs => 
-                                   let md := nth_error jr n in
-                                   iter_row rs match md with
-                                   | Some (data_node s) => 
-                                               match jt with
-                                               | None => Some (tmbranch [(k, tleaf s)])
-                                               | Some (tmbranch tm) => Some (tmbranch (app tm [(k, tleaf s)]))
-                                               | _ => jt
-                                               end
-                                   | Some root_node => let mt' := jtable_tree' n' n jr jtb in
-                                               match mt' with
-                                               | None => jt
-                                               | Some t' => 
-                                                 match jt with
-                                                 | None => Some (tmbranch [(k, t')])
-                                                 | Some (tmbranch tm) => Some (tmbranch (app tm [(k, t')]))
-                                                 | _ => jt
-                                                 end
-                                               end
-                                   | None => None
-                                   end
-            end in
-            let mjt' := iter_row r' None in
-            match mjt' with
-            | None => Some (tlbranch [])
-            | _ => mjt' 
-            end
-| None => None
-end
-end.
-
-Definition jtable_tree jr jtb := jtable_tree' ((length jr)*(length jr)) 0 jr jtb.
-
-Let t2:=(jtable_tree tn1 (snd jtb1)).
-Eval compute in t2.
-
-Example jtt_eq1: Some t1 = t2.
-Proof. auto. Qed.
-
-Definition clear_node_index (l: list indjnode) : jtable_row :=
-map (fun n => match n with
-| ind_data_node _ s => data_node s
-| ind_root_node _ _ => root_node
-end) l.
-
-Example jtt_eq2: tn1 = clear_node_index (fst jtb1).
-Proof. auto. Qed.
-
-Let json1 := {"menu" # {"header" # $"SVG Viewer",
-    "items" # '[
-        {"id"# $"Open"};
-        {"id"# $"OpenNew", "label"# $"Open New"};
-        {"id"# $"ZoomIn", "label"# $"Zoom In"};
-        {"id"# $"ZoomOut", "label"# $"Zoom Out"};
-        {"id"# $"OriginalView", "label"# $"Original View"};
-        {"id"# $"Quality"};
-        {"id"# $"Pause"};
-        {"id"# $"Mute"};
-        {"id"# $"Find", "label"# $"Find..."};
-        {"id"# $"FindAgain", "label"# $"Find Again"};
-        {"id"# $"Copy"};
-        {"id"# $"CopyAgain", "label"# $"Copy Again"};
-        {"id"# $"CopySVG", "label"# $"Copy SVG"};
-        {"id"# $"ViewSVG", "label"# $"View SVG"};
-        {"id"# $"ViewSource", "label"# $"View Source"};
-        {"id"# $"SaveAs", "label"# $"Save As"};
-        {"id"# $"Help"};
-        {"id"# $"About", "label"# $"About Adobe CVG Viewer..."}]}}.
-
-Let tree1 := json_tree json1.
-Let json11 := tree_json tree1.
-
-Example test1 : Some json1 = json11.
-Proof. auto. Qed.
-
-Let row1 := jtree_nodes tree1.
-Let table10 := jtable_fill (length row1) None.
-Let table1 := jtree_table tree1.
-Let tree11 := jtable_tree row1 (snd table1).
-
-Example test2 : Some tree1 = tree11.
-Proof. auto. Qed.
 
 Fixpoint find' (k: jpoint) (l: list (nat*option jpoint)) : option nat :=
 match l with
@@ -720,321 +114,6 @@ Eval compute in (find (inr 4) [None; None; Some (inl "foo"); Some (inr 4)]).
 Eval compute in (find (inl "foo") [None; None; Some (inl "foo"); Some (inr 4)]).
 Eval compute in (find (inr 14) [None; None; Some (inl "foo"); Some (inr 4)]).
 
-
-Fixpoint path_ind' (n:nat) (lk: jpath) (jr: list indjnode) (jtb: jtable) : 
-                                                  option (nat + nat*nat) :=
-match lk with
-| [] => let mv := nth_error jr n in
-        match mv with
-        | None => None
-        | Some (ind_data_node n _) => Some (inl n)
-        | Some (ind_root_node m n) => Some (inr (m, n))
-        end
-| k::ks => let mr := nth_error jtb n in
-           match mr with
-           | None => None
-           | Some r => let mn := find k r in
-                       match mn with
-                       | None => None
-                       | Some n => path_ind' n ks jr jtb
-                       end
-           end
-end.
-
-Definition tree_path_ind lk jt :=
-let (jr, tb) := jtree_table jt in
-path_ind' 0 lk jr tb.
-
-Eval compute in (tree_path_ind [inr 2; inl "baz"; inl "x"]
-                 (json_tree ('[{"foo" # '[$"Andy"; $"Peter"]}; 
-                    {"bar" # $"Good"};
-                    {"baz" # {"x" # '[$"d"; $"f"]}}]))).
-                    
-Eval compute in (tree_path_ind [inr 1; inl "bar"]
-                 (json_tree ('[{"foo" # '[$"Andy"; $"Peter"]}; 
-                    {"bar" # $"Good"};
-                    {"baz" # {"x" # '[$"d"; $"f"]}}]))).
-
-                    
-Eval compute in  (nth_error (snd (jtree_table
-                 (json_tree ('[{"foo" # '[$"Andy"; $"Peter"]}; 
-                    {"bar" # $"Good"};
-                    {"baz" # {"x" # '[$"d"; $"f"]}}])))) 8).
-
-
-Definition table_json_default jr tb j :=
-let mtr := jtable_tree jr tb in
-match mtr with
-| None => j
-| Some tr => let mj' := tree_json  tr in
-                         match mj' with
-                         | None => j
-                         | Some j' => j'
-                         end
-end.
-
-Definition mnth_error {X} (ll: list (list (option X))) m n : option X :=
-let ml := nth_error ll m in
-match ml with 
-| None => None
-| Some l => let mk := nth_error l n in
-            match mk with
-            | Some None => None
-            | Some x => x
-            | None => None
-            end
-end. 
-
-Fixpoint replaceSome {X} (l: list (option X)) x :=
-match l with 
-| [] => []
-| a::l' => if a then x::(replaceSome l' x)
-                else a::(replaceSome l' x)
-end.
-
-Definition json_rename (newv: data + key) (lk: jpath) (j: json) :=
-let tr := json_tree j in
-let (jr, tb) := jtree_table tr in
-let minds := tree_path_ind lk tr in
-match minds, newv with
-| None, _  => j
-| Some (inl k), inl newv => 
-                  let jr' := replace k (clear_node_index jr) (data_node newv) in
-                  table_json_default jr' tb j
-| Some (inl k), inr newv =>  let tb' := fold_right (fun m tb => let x := mnth_error tb m k in
-                                                                if x then jtable_set tb m k (Some (inl newv))
-                                                                     else tb) tb (seq 0 (length jr)) in
-                             table_json_default (clear_node_index jr) tb' j
-| Some (inr (m, n)), inr newv => 
-                  let tb' := jtable_set tb m n (Some (inl newv)) in
-                  table_json_default (clear_node_index jr) tb' j 
-| _, _ =>  j
-end.
-
-Example rename1: (json_rename (inr "y") [inr 2; inl "baz"; inl "x"]
-                  '[{"foo" # '[$"Andy"; $"Peter"]}; 
-                    {"bar" # $"Good"};
-                    {"baz" # {"x" # '[$"d"; $"f"]}}]    = 
-                   '[{"foo" # '[$"Andy"; $"Peter"]}; 
-                    {"bar" # $"Good"};
-                    {"baz" # {"y" # '[$"d"; $"f"]}}]).
-Proof. auto. Qed.
-
-Example rename2: (json_rename (inl "Mike") [inr 0; inl "foo"; inr 0]
-                  '[{"foo" # '[$"Andy"; $"Peter"]}; 
-                    {"bar" # $"Good"};
-                    {"baz" # {"x" # '[$"d"; $"f"]}}] = 
-                   '[{"foo" # '[$"Mike"; $"Peter"]}; 
-                    {"bar" # $"Good"};
-                    {"baz" # {"x" # '[$"d"; $"f"]}}]).
-Proof. auto. Qed.
-
-Example rename3: json_rename (inr "y") [inr 1; inl "bar"]
-                  '[{"foo" # '[$"Andy"; $"Peter"]}; 
-                    {"bar" # $"Good"};
-                    {"baz" # {"x" # '[$"d"; $"f"]}}] = 
-                    '[{"foo" # '[$"Andy"; $"Peter"]}; 
-                    {"y" # $"Good"};
-                    {"baz" # {"x" # '[$"d"; $"f"]}}].
-Proof. auto. Qed.
-
-Let json2 := '[{"type" # $"person",
-                "name" # '[{"given" # '[$"Andy"; $"Michael"], "family" # $"Watson"};
-                            {"given" # '[$"Andrey"], "family" # $"Watsonov"}],
-                "telecom" # '[{"system" # $"phone", "value" # $"1234"};
-                              {"system" # $"phone", "value" # $"5678"};
-                              {"system" # $"mail", "value" # $"andy@watson.me"};
-                              {"system" # $"mail", "value" # $"andrey@mail.ru"}]
-                 };
-                {"type" # $"person",
-                "name" # '[{"given" # '[$"John"; $"Israel"], "family" # $"Koen"};
-                            {"given" # '[$"Ivan"], "family" # $"Koinov"}],
-                "telecom" # '[{"system" # $"phone", "value" # $"4321"};
-                              {"system" # $"phone", "value" # $"8765"};
-                              {"system" # $"mail", "value" # $"john@koen.me"}]
-                }].
-
-Let json3 := '[{"given1" # $"Andy Michael", "family1" # $"Watson",
-                "given2" # $"Andrey", "family2" #  $"Watsonov",
-                "phone1" # $"1234", "phone2" # $"5678",
-                "mail1" # $"andy@watson.me",
-                "mail2" # $"andrey@mail.ru"};
-                {"given1" # $"John Israel", "family1" # $"Koen",
-                "given2" # $"Ivan", "family2" #  $"Koinov",
-                "phone1" # $"4321", "phone2" # $"8765",
-                "mail1" # $"john@koen.me"}].
-
-
-Inductive DestructStrategy := DestructStrategy0.
-
-Inductive IndMergeStrategy := 
-| IndRightMergeToNumber : IndMergeStrategy
-| IndRightMergeToKey : (key -> key) -> IndMergeStrategy.
-
-Fixpoint merge_inds (ilt ilf: list (option jpoint)) 
-                    (s:IndMergeStrategy) (b: bool):=
-match ilt, ilf with
-| [], ilf' => ilf'
-| ilt', [] => ilt'
-| None::ilt', (Some x)::ilf' => let l := merge_inds ilt' ilf' s b in
-                         match x, s with
-                         | inl kx, IndRightMergeToNumber => (Some (inr 0))::l
-                         | inr ix, IndRightMergeToNumber => (Some x)::l
-                         | inl kx, IndRightMergeToKey f => (Some (inl (f kx)))::l
-                         | inr ix, IndRightMergeToKey f => (Some (inl (f (writeNat ix))))::l
-                         end
-| x::ilt', None::ilf' => x::(merge_inds ilt' ilf' s b)
-(*shouldn't be happened*)
-| (Some x)::ilt',(Some y)::ilf' => 
-                            let z:= match x,y with
-                                    | inl kx, inl ky => inl (kx ++ "." ++ ky)
-                                    | inl kx, inr iy => inl (kx ++ "." ++ (indexNat iy))
-                                    | inr ix, inl ky => inr ix (*FIXME:will be ignored, but...*)
-                                    | inr ix, inr iy => inr ix (*FIXME:will be ignored, but...*)
-                                    end in
-                            if b then (Some x)::(merge_inds ilt' ilf' s b)
-                                 else (Some z)::(merge_inds ilt' ilf' s b)
-end.
-
-Definition json_destruct (lk: jpath) (j: json): json :=
-let tr := json_tree j in
-let (jr, tb) := jtree_table tr in
-let minds := tree_path_ind lk tr in
-match minds with
-| None => j
-| Some (inl k) => let tb' := fold_right (fun m tb => jtable_set tb m k None) 
-                                          tb (seq 0 (length jr)) in
-                  table_json_default (clear_node_index jr) tb' j 
-
-| Some (inr (m, n)) => let milt := nth_error tb m in
-                       let milf := nth_error tb n in
-                       let mtr := tree_getin (removelast lk) tr in
-                       let last := last lk (inl "") in
-                       let slast := match last with
-                                    | inr k => writeNat k
-                                    | inl k => k
-                                    end in
-                       match milt, milf, mtr with
-                           | None, _, _ => j
-                           | _, None, _ => j
-                           | _, _, None => j
-                           | _, _, Some (tleaf _) => j
-                           | Some ilt, Some ilf, Some (tlbranch _)  => 
-                                       let ilt' := merge_inds ilt ilf IndRightMergeToNumber true in
-                                       let tb' := replace m tb ilt' in
-                                       let tb'' := jtable_set tb' m n None in
-                                       table_json_default (clear_node_index jr) tb'' j
-                           | Some ilt, Some ilf, Some (tmbranch _)  => 
-                                       let ilt' := merge_inds ilt ilf (IndRightMergeToKey (fun k => (append (append slast "-") k))) true in
-                                       let tb' := replace m tb ilt' in
-                                       let tb'' := jtable_set tb' m n None in
-                                       table_json_default (clear_node_index jr) tb'' j
-                       end
-end.
-
-Definition json_remove (lk: jpath) (j: json): json :=
-let tr := json_tree j in
-let (jr, tb) := jtree_table tr in
-let minds := tree_path_ind lk tr in
-match minds with
-| None => j
-| Some (inl k) => let tb' := fold_right (fun m tb => jtable_set tb m k None) 
-                                          tb (seq 0 (length jr)) in
-                  table_json_default (clear_node_index jr) tb' j 
-
-| Some (inr (m, n)) => let tb' := jtable_set tb m n None in
-                       table_json_default (clear_node_index jr) tb' j
-                           
-end.
-
-Definition json_modify (f: jtree -> jtree) (lk: jpath) (j: json) : json :=
-let tr := json_tree j in
-let tr' := tree_modify lk tr f in
-let mj' := tree_json tr' in
-match mj' with
-| None => j
-| Some j' => j'
-end.
-
-Let tree2 := json_tree json2.
-Let tb22 := jtree_table tree2.
-Let tab2 := snd tb22.
-
-Fixpoint split_string' (s: string) (p: string) n : list string :=
-match n with
-| O => []
-| S n' => 
-if (string_dec s "") then [] else
-if (string_dec p "") then (substring 0 1 s)::
-                          (split_string' (substring 1 ((String.length s) - 1) s) p n') else
-let i := index 0 p s in
-match i with
-| None => [s]
-| Some k => let ss := substring 0 k s in
-            let a  := k + (String.length p) in
-            let s' := substring a ((String.length s) - a) s in
-            ss::(split_string' s' p n')
-end
-end.
-
-Definition split_string s p := split_string' s p (String.length s). 
-
-
-Definition split_tree_with (d: data) (jt: jtree): jtree :=
-match jt with
-| tleaf s => let ss := split_string s d in
-             tlbranch (indexate (map (@tleaf data key) ss))
-| _ => jt (* FIXME *)
-end.
-
-Eval compute in (split_string "a.b.c.*" ".").
-Eval compute in (split_string "aaaa" ".").
-Eval compute in (split_string "." ".").
-Eval compute in (split_string "aaaa" "").
-Eval compute in (split_string ".aaa.a.e." ".").
-
-Require Import String Ascii.
-Definition num_of_ascii (c: ascii) : option nat :=
- match c with
-(* Zero is 0011 0000 *)
-   | Ascii false false false false true true false false => Some 0
-(* One is 0011 0001 *)
-   | Ascii true false false false true true false false => Some 1
-(* Two is 0011 0010 *)
-   | Ascii false true false false true true false false => Some 2
-   | Ascii true true false false true true false false => Some 3
-   | Ascii false false true false true true false false => Some 4
-   | Ascii true false true false true true false false => Some 5
-   | Ascii false true true false true true false false => Some 6
-   | Ascii true true true false true true false false => Some 7
-   | Ascii false false false true true true false false => Some 8
-   | Ascii true false false true true true false false => Some 9
-   | _ => None
-end.
-
-Fixpoint string_rev (s : string) : string :=
- match s with
- | EmptyString => EmptyString
- | String c rest => append (string_rev rest) (String c EmptyString)
-end.
-
-Fixpoint num_of_string_rec (s : string) : option nat :=
-  match s with
-    | EmptyString => Some 0
-    | String c rest => 
-       match (num_of_ascii c), (num_of_string_rec rest) with
-          | Some n, Some m => Some (n + 10 * m)
-          | _ , _ => None
-       end
-   end.
-
-Definition num_of_string (s : string) := 
-  num_of_string_rec (string_rev s).
-
-Eval compute in num_of_string "1".
-Eval compute in num_of_string "10".
-Eval compute in num_of_string "174".
-
 Definition from_string (s: string) : jpoint :=
 if (prefix "#" s) then 
 let mk := num_of_string (substring 1 (String.length s -1) s) in
@@ -1049,202 +128,6 @@ Eval compute in (from_string "#4t").
 Eval compute in (from_string "").
 Eval compute in (from_string "foo").
 
-Check tree_getin.
-
-Fixpoint filterSome {X} (l: list (option X)) : list X :=
-match l with
-| [] => []
-| None::xs => filterSome xs
-| (Some x) :: xs => x::(filterSome xs)
-end.
-
-Check tree_get.
-
-Definition remove_prefix (p s: string) : string :=
-if (prefix p s) then substring (String.length p) ((String.length s) - (String.length p)) s
-else s.
-
-Eval compute in (remove_prefix "ddd" "dddpol").
-Eval compute in (remove_prefix "" "dddpol").
-Eval compute in (remove_prefix "dddr" "dddpol").
-
-Print string.
-
-Fixpoint bany (l: list bool): bool :=
-match l with
-| [] => false
-| true::_ => true
-| _::l' => bany l'
-end.
-
-Fixpoint substrings (s: string): list string :=
-match s with
-| EmptyString => [EmptyString]
-| String c s' => s::(substrings s')
-end.
-
-Eval compute in (substrings "abc").
-
-Eval compute in (match "*" with
-                 | String c s => Some c
-                 | _ => None
-                 end).
-
-Print ascii.
-
-Fixpoint match_string (p s: string): bool :=
-match p, s with
-| EmptyString, EmptyString => true
-| String ("*"%char) xp, EmptyString => match_string xp EmptyString
-| String ("*"%char) xp, String cs xs => bany (map (match_string xp) (substrings s))
-| String cp xp, String cs xs => if (string_dec (String cp EmptyString)
-                                               (String cs EmptyString)) then 
-                                match_string xp xs else false
-| _, _ => false
-end.
-
-Eval compute in (match_string "abc" "abc").
-Eval compute in (match_string "abcd" "abc").
-Eval compute in (match_string "abc" "abcd").
-Eval compute in (match_string "abc*" "abc").
-Eval compute in (match_string "abc*ijh" "abcdefijh").
-Eval compute in (match_string "abc*ijh*" "abcdefijh").
-Eval compute in (match_string "abc*" "abcdefijh").
-Eval compute in (match_string "*" "abcdefijh").
-Eval compute in (match_string "" "abcdefijh").
-Eval compute in (match_string "a" "abcdefijh").
-
-Check filter.
-
-Definition tree_wild_get (p: jpoint) (jpt: jpath*jtree): list (jpath*jtree) :=
-let (p0, jt) := jpt in
-match p with
-| inr k => let mt := tree_get p jt in
-           match mt with
-           | None => []
-           | Some (_, t) => [(app p0 [p], t)]
-           end
-| inl k => match jt with
-           | tleaf s => []
-           | tlbranch tl => map (fun kt => (app p0 [inr (fst kt)], snd kt))
-                            (filter (fun (kt:nat*jtree) => let (k', t) := kt in
-                                     match_string k (indexNat k')) tl)
-           | tmbranch tm => map (fun kt => (app p0 [inl (fst kt)], snd kt))
-                            (filter (fun (kt:key*jtree) => let (k', t) := kt in
-                                     match_string k k') tm)
-           end
-end.
-
-
-Definition path_tree (ls: list string) root jt : list jpath :=
-let mt := tree_getin root jt in 
-match mt with 
-| None => []
-| Some jt => let jts := fold_right (fun s jts => let mts := map (tree_wild_get (from_string s)) jts in
-                                    let ts := flatten mts in
-                                    ts) [([],jt)] ls in
-                        map (fun p => app root (fst p)) jts
-end.
-
-Definition path_parse (s: string) (root: jpath) jt : list jpath :=
-let ls := split_string s "." in
-path_tree (rev ls) root jt.
-
-Definition do_at_nodes (j: json) (f: jpath -> json -> json) (path: string) : json :=
-let jt := json_tree j in
-let llk := path_parse path [] jt in
-fold_right f j llk. 
-
-Eval compute in (path_parse "*.name" [] tree2).
-
-Let json21' := do_at_nodes json2 json_destruct "*.name".
-Eval compute in json21'.
-Eval compute in (json_getin [inr 0; inl "name-0"] json21').
-Eval compute in (json_getin [inr 0; inl "name-1"] json21').
-Let json22' := do_at_nodes json21' json_destruct "*.name*".
-Eval compute in json22'.
-Let json23' := do_at_nodes json22' (json_modify (concat_tree_with " ")) "*.name*given".
-Eval compute in json23'.
-Let json24' := do_at_nodes json23' json_destruct "*.telecom".
-Eval compute in json24'.
-Let json25' := do_at_nodes json24' (json_modify (fun t => let mt1 := tree_getin [inl "system"] t in
-                                                             let mt2 := tree_getin [inl "value"] t in
-                                                             match mt1, mt2 with
-                                                             | Some (tleaf s1), Some (tleaf s2) => 
-                                                                    (tmbranch [(s1, tleaf s2)])
-                                                             | _, _ => t
-                                                             end))  "*.telecom*".
-Eval compute in json25'.
-Let json26' := do_at_nodes json25' json_destruct "*.telecom*".
-Eval compute in json26'.
-Let json27' := do_at_nodes json26' (json_rename (inr "given1")) "*.name-0-given".
-Let json28' := do_at_nodes json27' (json_rename (inr "given2")) "*.name-1-given".
-Let json29' := do_at_nodes json28' (json_rename (inr "family1")) "*.name-0-family".
-Let json210' := do_at_nodes json29' (json_rename (inr "family2")) "*.name-1-family".
-Let json211' := do_at_nodes json210' (json_rename (inr "phone1")) "*.telecom-0-phone".
-Let json212' := do_at_nodes json211' (json_rename (inr "phone2")) "*.telecom-1-phone".
-Let json213' := do_at_nodes json212' (json_rename (inr "mail1")) "*.telecom-2-mail".
-Let json214' := do_at_nodes json213' (json_rename (inr "mail2")) "*.telecom-3-mail".
-Let json215' := do_at_nodes json214' json_destruct "*.type".
-
-Example mapping1 : json3 = json215'.
-Proof. compute. auto. Qed.
-
-(*CREATE AT "*.telecom"*)
-Definition json_create (s: string) (lk: jpath) (j: json) : json :=
-let jt := json_tree j in
-let p := from_string s in
-let mjt' := tree_getin lk jt in
-let jt' := match mjt' with 
-| None => jt
-| Some jt' => let mjt'' := tree_get p jt' in
-              let pth := app lk [p] in
-              match mjt'' with
-              | Some _ => jt
-              | None => match p with
-                        | inr k => tree_mergein lk jt (tlbranch [(k, tlbranch [])]) MergeStrategy0
-                        | inl k => tree_mergein lk jt (tmbranch [(k, tlbranch [])]) MergeStrategy0
-                        end
-              end
-end in
-(*let jt' := fold_right (fun p (pjt: jpath*jtree) => let (pth, jt) := pjt in
-                                    let pth' := app pth [p] in
-                                    let mjt' := tree_getin pth' jt in
-                                    match mjt' with
-                                    | Some _ => (pth', jt)
-                                    | None => match p with
-                                              | inr k => (pth', tree_mergein pth jt (tlbranch [(k, tlbranch [])]) MergeStrategy0)
-                                              | inl k => (pth', tree_mergein pth jt (tmbranch [(k, tlbranch [])]) MergeStrategy0)
-                                              end
-                                    end) ([], jt) lk in*)
-let mj' := tree_json jt' in
-match mj' with
-| None => j
-| Some j' => j'
-end.
-
-Check fold_left.
-(*fold_left
-     : forall A B : Type,
-       (A -> B -> A) ->
-       list B -> A -> A*)
-
-(* COLLECT "telecom*" TO "telecom" AT "*" *)
-Definition json_collect (what pto: string) f (root: jpath) (j: json) : json :=
-let jt := json_tree j in
-let llkf := path_parse what root jt in
-let llkt := path_parse pto root jt in
-let jt' := fold_left (fun jt lkf => 
-                        fold_right (fun lkt jt => tree_submerge_with lkt lkf f jt MergeStrategy0) jt llkt) llkf jt in
-let mj' := tree_json jt' in
-match mj' with
-| None => j
-| Some j' => j'
-end.
-
-Check last.
-
-SearchAbout (key + nat -> string).
 
 Definition writeJPoint (p: jpoint) : string :=
 match p with
@@ -1252,215 +135,85 @@ match p with
 | inl k => k
 end.
 
-Check nth.
+Section json_ind'.
 
-Definition map_tree_with_old (ks: list key) (jt: jtree) : jtree :=
-match jt with
-| tleaf _ => jt
-| tlbranch tl => tlbranch (indexate (map (fun (ks:nat*key) => let (k,s):=ks in 
-                                let txs := filterSome (map (tree_get (inr k)) (map snd tl)) in
-                                tmbranch [(s, tlbranch txs)] ) (indexate ks)))
-| _ => jt
+Check json_ind.
+
+Variable P: json -> Prop.
+
+Hypothesis json_data_case : forall (dj : JsonData),
+    P (json_data dj).
+
+Hypothesis json_list_case : forall (lj : list json),
+    Forall P lj -> P (json_list lj).
+
+Hypothesis json_map_case : forall (mj : @key_map json),
+    Forall P (keymap_list mj) -> P (json_map mj).
+
+
+Fixpoint json_ind' (j : json) : P j :=
+match j return (P j) with
+| $s => json_data_case  s
+| ' lj => json_list_case lj
+        ((fix json_list_ind (lj : list json) : Forall P lj :=
+          match lj with
+            | [] => Forall_nil P
+            | j::ljx => @Forall_cons json P j ljx (json_ind' j) (json_list_ind ljx)
+          end) lj)
+| & mj => json_map_case mj
+        ((fix json_map_ind (mj : @key_map json) : Forall P (keymap_list mj) :=
+          match mj with
+            | empty => Forall_nil P
+            | mapkv k v mjx => @Forall_cons json P v (keymap_list mjx) (json_ind' v) (json_map_ind mjx)
+          end) mj)
 end.
 
-(*
-(("name") # (' [' [' [$ "Andy"; $ "Michael"]; $ "Watson"];
-                ' [' [$ "Andrey"]; $ "Watsonov"]])
-*)
-Fixpoint zip_first_with {X Y T} (ks: list X) (lxy: list (T*Y)) d (f: T->X): list (X*Y) :=
-match ks, lxy with
-| [], _ => map (fun (ky:T*Y) => let (k,y):= ky in (f k,y)) lxy
-| _, [] => map (fun k => (k,d)) ks
-| k::kss, (x,y)::lxys => (k,y)::(zip_first_with kss lxys d  f)
-end.
+End json_ind'.
 
+Check json_ind'.
 
-Definition zip_tree_with (ks: list key) (jt: jtree) : jtree :=
-match jt with
-| tleaf _ => jt
-| tlbranch tl => tmbranch (zip_first_with ks tl (tlbranch []) indexNat)
-| tmbranch tm => tmbranch (zip_first_with ks tm (tlbranch []) (@id key))
-end.
+(*tests*)
 
-Definition map_tree_with (ks: list key) (jt: jtree) : jtree :=
-match jt with
-| tleaf _ => jt
-| tlbranch tl => tlbranch (map (fun (kt:nat*jtree) => let (k,t) := kt in  
-                                          (k, zip_tree_with ks t)) tl)
-| tmbranch tm => tmbranch (map (fun (kt:key*jtree) => let (k,t) := kt in  
-                                          (k, zip_tree_with ks t)) tm)
-end.
+Check ($"foo").
+Check {"foo" # $"bar"}.
+Check ('([$"foo"]%list)).
+Check {"1" # $"Andy" , "2" # $"Peter"}.
 
+Let json1 := {"foo" # $"Andy", "bar" #  $"Peter"}.
+Let json2 := '[$"Andy"; $"Peter"].
 
-Fixpoint ziplists' {X} (ll : list (list X))  (l: list X) :=
-match ll, l with
-| _, [] => ll
-| [], x::xs => map (fun x => [x]) l
-| lx::lxs, x::xs => (app lx [x])::(ziplists' lxs xs)
-end.
+Eval compute in (jsonmap (fun x => {}) {"foo" # $"foo", "bar" # $"bar"}).
 
-Eval compute in (ziplists' [[1;2]; [3;4]] [5;6;7;8]).
-Eval compute in (ziplists' [] [5;6;7;8]).
+Example json_get1: json_get (inl "foo") json1 = Some $"Andy".
+Proof. auto. Qed.
 
-Definition ziplists {X} (ll : list (list X)) :=
- fold_left ziplists' ll [].
- 
-Eval compute in (ziplists [[1;2]; [3;4]; [5;6;7;8]]).
-Fixpoint ziptrees' (ll : list jtree)  (l: jtree) :=
-match ll, l with
-| _, tlbranch [] => ll
-| [], tlbranch ((_::_) as l) => map (fun x => tlbranch [x]) l
-| (tlbranch lx)::lxs, tlbranch (x::xs) => (tlbranch (app lx [x]))::(ziptrees' lxs (tlbranch xs))
-| _,_ => ll
-end.
+Example json_get2: json_get (inl "bar") json1 = Some $"Peter".
+Proof. auto. Qed.
 
-Definition json_zip_at (ks: list string) (root: jpath) (j: json) :=
-let jt := json_tree j in
-let llkf := flatten (map (fun s => path_parse s root jt) ks) in
-let trees := filterSome (map (fun p => tree_getin p jt) llkf) in 
-let jt' := tree_setin root jt (tlbranch (indexate (fold_left ziptrees' trees []))) in
-let mj' := tree_json jt' in
-match mj' with
-| None => j
-| Some j' => j'
-end.
+Example json_get3: json_get (inl "baz") json1 = None.
+Proof. auto. Qed.
 
+Example json_get4: json_get (inr 0) json2 = Some $"Andy".
+Proof. auto. Qed.
 
-Let json31' := do_at_nodes json3 (json_create "type") "*".
-Let json32' := do_at_nodes json31' (json_modify (fun _ => tleaf "person")) "*.type".
-Eval compute in json32'.
+Example json_get5: json_get (inr 1) json2 = Some $"Peter".
+Proof. auto. Qed.
 
-Let json33' := do_at_nodes json32' (json_rename (inr "name-0-given")) "*.given1".
-Let json34' := do_at_nodes json33' (json_rename (inr "name-1-given")) "*.given2".
-Let json35' := do_at_nodes json34' (json_rename (inr "name-0-family")) "*.family1".
-Let json36' := do_at_nodes json35' (json_rename (inr "name-1-family")) "*.family2".
-Let json37' := do_at_nodes json36' (json_rename (inr "telecom-0-phone")) "*.phone1".
-Let json38' := do_at_nodes json37' (json_rename (inr "telecom-1-phone")) "*.phone2".
-Let json39' := do_at_nodes json38' (json_rename (inr "telecom-2-mail")) "*.mail1".
-Let json310' := do_at_nodes json39' (json_rename (inr "telecom-3-mail")) "*.mail2".
+Example json_get6: json_get (inr 2) json2 = None.
+Proof. auto. Qed.
 
-Let json311' := do_at_nodes json310' (json_modify (split_tree_with " ")) "*.name*given".
-Eval compute in json311'.
-Let json312' := do_at_nodes json311' (json_create "'name-given") "*".
-Let json313' := do_at_nodes json312' (json_collect "name*given" "'name-given" (fun lk jt => tlbranch [(0, jt)])) "*".
-Eval compute in json313'.
-Let json314' := do_at_nodes json313' (json_create "'name-family") "*".
-Let json315' := do_at_nodes json314' (json_collect "name*family" "'name-family" (fun lk jt => tlbranch [(0, jt)])) "*".
-Eval compute in json315'.
-Let json316' := do_at_nodes json315' json_remove "*.name*".
-Eval compute in json316'.
-Let json317' := do_at_nodes json316' (json_create "name") "*".
-Let json318' := do_at_nodes json317' (json_collect "'name*" "name" (fun lk jt => let l := last lk (inl "error") in
-                                                                                 let sl := writeJPoint l in
-                                                                                 let sl' := split_string sl "-" in
-                                                                                 let sl'' := nth 1 sl' "error" in
-                                                                    tmbranch [(sl'', jt)])) "*".
-Eval compute in json318'.
-Let json319' := do_at_nodes json318' json_remove "*.'name*".
-Eval compute in json311'.
-Let json320' := do_at_nodes json319' (json_zip_at ["given"; "family"]) "*.name".
-Eval compute in json320'.
-Let json321' := do_at_nodes json320' (json_modify (map_tree_with ["given"; "family"])) "*.name".
-Eval compute in json321'.
+Example json_getin1:  json_getin [inl "foo"; inr 1] {"foo" # json2} = Some $"Peter".
+Proof. auto. Qed.
 
-Let json322' := do_at_nodes json321' (json_create "'telecom") "*".
-Let json323' := do_at_nodes json322' (json_collect "telecom*" "'telecom" (fun lk jt => let l := last lk (inl "error") in
-                                                                                      let sl := writeJPoint l in
-                                                                                      let sl' := split_string sl "-" in
-                                                                                      let sl'' := last sl' "error" in
-                                                                        tlbranch [(0, tmbranch [("system", tleaf sl''); 
-                                                                                  ("value", jt)])])) "*".
-Eval compute in json323'.
-Let json324' := do_at_nodes json323' json_remove "*.telecom*".
-Eval compute in json324'.
-Let json325' := do_at_nodes json324' (json_rename (inr "telecom")) "*.'telecom".
-Eval compute in json325'.
+(*lemmas*)
 
-Example mapping2 : json2 = 
-                   json325'.
-Proof. compute. auto. Qed.
-(*
-DO_SMTH BY_METHOD WITH_PARAM AT_PATH
-json2 -> json3
+Lemma json_get1_data_none: forall k s, json_get (inr k) $s = None.
+Proof.
+ intros. simpl. auto. Qed.
 
-REMOVE (by purge) "type" AT ".*" -- all rooted collection
-
-
--- {"name" # '[{"given" # '[$"Andy"; $"Michael"], "family" # $"Watson"};
-               {"given" # '[$"Andrey"], "family" # $"Watsonov"}]}
-
-DESTRUCT (by disjoin, indexate) AT ".*.name"  -- on lists
--- "name1" # {"given" # '[$"Andy"; $"Michael"], "family" # $"Watson"}
--- "name2" # {"given" # '[$"Andrey"], "family" # $"Watsonov"}
-
-DESTRUCT (by renaming, indexate key???) AT ".*.name*" -- on maps
--- {"given1" # '[$"Andy"; $"Michael"], "family1" # $"Watson",
---  "given2" # '[$"Andrey"], "family2" # $"Watsonov"}
-
-DESTRUCT (by concat, with delimiter " ") AT ".*.given*" -- on  lists
--- {"given1" # $"Andy Michael"], "family1" # $"Watson",
---  "given2" # $"Andrey", "family2" # $"Watsonov"}
-
--- {"telecom" # '[{"system" # $"phone", "value" # $"1234"};
---                {"system" # $"phone", "value" # $"5678"};
---                {"system" # $"mail", "value" # $"andy@watson.me"};
---                {"system" # $"mail", "value" # $"andrey@mail.ru"}]}
-
-DESTRUCT (by disjoin, indexate) AT ".*.telecom" -- on lists
--- {"telecom1" # {"system" # $"phone", "value" # $"1234"},
---  "telecom2" # {"system" # $"phone", "value" # $"5678"},
---  "telecom3" # {"system" # $"mail", "value" # $"andy@watson.me"},
---  "telecom4" # {"system" # $"mail", "value" # $"andrey@mail.ru"}}
-
-SET (by replace with map {@"system" # @"value"}) AT ".*.telecom*" -- on maps
--- {"telecom1" # {"phone" # $"1234"},
---  "telecom2" # {"phone" # $"5678"},
---  "telecom3" # {"mail"  # $"andy@watson.me"},
---  "telecom4" # {"mail"  # $"andrey@mail.ru"}}
-
-DESTRUCT (by renaming, indexate key???) AT ".*.telecom*" -- on maps
--- {"phone1" # $"1234",
---  "phone2" # $"5678",
---  "mail1"  # $"andy@watson.me",
---  "mail2"  # $"andrey@mail.ru"}
-
-*)
-
-(*
-json3 -> json2
--- {"phone1" # $"1234", "phone2" # $"5678",
---  "mail1" # $"andy@watson.me",
---  "mail2" # $"andrey@mail.ru"}
-
-SET (by destruct_insert of values ".*.phone*") AT ".*.phones"
-SET (by destruct_insert of values ".*.mail*") AT ".*.mails"
--- {"phones" # '[$"1234"; $"5678"],
---  "mails"  # '[$"andy@watson.me"; $"andrey@mail.ru"]}
-
-SET (by replace with map {"system" # $"phone", "value" # @id}) AT ".*.phones.*"
-SET (by replace with map {"system" # $"mail", "value" # @id}) AT ".*.mails.*"
--- {"phones" # '[{"system" # $"phone", "value" # $"1234"}; 
---               {"system" # $"phone", "value" # $"5678"}],
---  "mails"  # '[{"system" # $"mail", "value"$"andy@watson.me"}; 
---               {"system" # $"mail", "value"$"andrey@mail.ru"}]}
-
-SET (by destruct_insert of values [".*.mails", ".*.phones"]) AT ".*.telecom"
--- {"telecom" # '['[{"system" # $"phone", "value" # $"1234"}; 
---               {"system" # $"phone", "value" # $"5678"}];
---              '[{"system" # $"mail", "value"$"andy@watson.me"}; 
---               {"system" # $"mail", "value"$"andrey@mail.ru"}]]}
-
-SET (by replace with map flatten) AT ".*.telecom"
--- {"telecom" # '[{"system" # $"phone", "value" # $"1234"}; 
---               {"system" # $"phone", "value" # $"5678"};
---               {"system" # $"mail", "value"$"andy@watson.me"}; 
---               {"system" # $"mail", "value"$"andrey@mail.ru"}]}
-*)
-
-
-
-
-
+Lemma json_get2_data_none: forall k s, json_get (inl k) $s = None.
+Proof.
+ intros. simpl. auto. Qed.
 
 
 
