JsonTable.v
@@ -1,0 +1,393 @@
+Require Import String.
+Require Import Lists.List.
+Require Import Coq.Init.Nat.
+Require Import Coq.Program.Basics.
+
+Require Export Json.
+Require Export JsonTree.
+
+Import ListNotations.
+Import JsonNotations.
+
+Local Open Scope list_scope.
+Local Open Scope string_scope.
+Local Open Scope json_scope.
+
+
+Definition jtable := list (list (option jpoint)). 
+
+Fixpoint list_fill {X} (n: nat) (x:X): list X :=
+match n with
+| O => []
+| S n' => x::(list_fill n' x)
+end.
+
+Definition jtable_fill (n: nat) (a: option jpoint): jtable:=
+list_fill n (list_fill n None).
+
+Definition jtable_set (jt: jtable) (m n: nat) (a: option jpoint) : jtable :=
+let ml := nth_error jt m in
+match ml with
+| Some l => replace m jt (replace n l a)
+| None => jt
+end.
+
+Inductive indjnode := 
+| ind_data_node: nat -> JsonData -> indjnode
+| ind_root_node: nat -> nat -> indjnode.
+
+Definition nlj_type := (nat*(list indjnode)*jtable)%type.
+
+Check fold_left.
+(*fold_left
+     : forall A B : Type,
+       (A -> B -> A) ->
+       list B -> A -> A*)
+
+(*fold_right (B -> A -> A) ->
+       A -> list B -> A*)
+
+Print fold_right.
+
+(*Lemma fst_fold_assoc: forall A1 A2 B (f:A1*A2->B->A1*A2) a l, fst (fold_left f l a) = fold_left (fun a b => fst (f a b)) l (fst a).*)
+
+Fixpoint jtree_table' (m: nat) (k: option jpoint) (jt: jtree)  
+                      (nlj: nlj_type) {struct jt}: nlj_type :=
+let (nl, jtb) := nlj in
+let (n, jr) := nl in
+match jt with
+| tleaf s => let newtb := jtable_set jtb m n k in
+             (S n, app jr [ind_data_node n s] , newtb)
+| tlbranch tl => fold_left (fun nlj kt => jtree_table' n (Some (inr (fst kt))) (snd kt) nlj) 
+                            tl (S n, app jr [ind_root_node m n], jtable_set jtb m n k)
+
+(*let newtb':= jtable_set jtb m n k in
+                 let jr' := app jr [ind_root_node m n] in
+                 let fix iter_tree m k tl nlj {struct tl}:=
+                 match tl with
+                 | [] => nlj
+                 | (a,t)::ts => iter_tree m None ts (jtree_table' m (Some (inr a)) t nlj)
+                 end in
+                 iter_tree n k tl (S n, jr', newtb')*)
+| tmbranch tm => fold_left (fun nlj kt => jtree_table' n (Some (inl (fst kt))) (snd kt) nlj) 
+                            tm (S n, app jr [ind_root_node m n], jtable_set jtb m n k)
+(*let newtb':= jtable_set jtb m n k in
+                 let jr' := app jr [ind_root_node m n] in
+                 let fix iter_tree m k tm nlj {struct tm}:=
+                 match tm with
+                 | [] => nlj
+                 | (a,t)::ts => iter_tree m None ts (jtree_table' m (Some (inl a)) t nlj)
+                 end in
+                 iter_tree n k tm (S n, jr', newtb')*)
+end.
+
+Definition jtree_table jt := let tb3 := jtree_table' 0 None jt (0, [],  
+                             (jtable_fill (length (jtree_nodes jt)) None)) in
+                             (snd (fst tb3), snd tb3).
+
+Definition clear_node_index (l: list indjnode) : jtable_row :=
+map (fun n => match n with
+| ind_data_node _ s => data_node s
+| ind_root_node _ _ => root_node
+end) l.
+
+Lemma clear_node_index_cons: forall a l, clear_node_index (a::l) = app (clear_node_index [a]) (clear_node_index l).
+Proof.
+ intros. generalize dependent a. induction l; intros.
+ simpl. destruct a; auto.
+ simpl. destruct a; destruct a0; auto.
+Qed.
+
+Lemma clear_node_index_app: forall a l, clear_node_index (app a l) = app (clear_node_index a) (clear_node_index l).
+Proof.
+ intros. generalize dependent l. induction a; intros.
+ simpl. auto.
+ simpl. destruct a. rewrite IHa. auto.
+ rewrite IHa. auto.
+Qed.
+
+Lemma one_tree_row: forall m m' n n' jtb jtb' k t jr jr' jr'', 
+clear_node_index (app jr jr') = clear_node_index jr'' ->
+app (clear_node_index jr) (clear_node_index (snd (fst (jtree_table' m' k t (n', jr', jtb'))))) =
+clear_node_index (snd (fst (jtree_table' m k t (n, jr'', jtb)))).
+Proof.
+ intros.  generalize dependent jr. generalize dependent jr'. 
+ generalize dependent jr''. generalize dependent jtb.
+ generalize dependent jtb'. generalize dependent n. generalize dependent n'.
+ generalize dependent m. generalize dependent m'.
+ generalize dependent k.
+ induction t using tree_ind'; intros.
+ simpl. rewrite 2 clear_node_index_app. simpl.
+ rewrite clear_node_index_app in H.
+ rewrite <- H. apply app_assoc.
+ 
+ simpl.
+ remember (S n') as n'1. remember (app jr' [ind_root_node m' n']) as jr'1.
+ remember (jtable_set jtb' m' n' k) as jtb'1.
+ remember (S n) as n1. remember (app jr'' [ind_root_node m n]) as jr''1.
+ remember (jtable_set jtb m n k) as jtb1. 
+ assert (clear_node_index (jr ++ jr'1) = clear_node_index jr''1).
+ subst. rewrite 3 clear_node_index_app. simpl. 
+ rewrite <- H0. rewrite clear_node_index_app. apply app_assoc.
+ generalize H1.
+ generalize jr'1.
+ generalize jr''1. generalize jtb1.
+ generalize jtb'1. generalize n'1. 
+ generalize n1. generalize n'. generalize n.
+ induction lj; intros. simpl.
+ rewrite <- clear_node_index_app. auto. simpl.
+ destruct a. replace (map snd ((n3, t) :: lj)) with
+ (t :: map snd lj) in H; auto. inversion H. clear H.
+ simpl. 
+ remember (jtree_table' n'0 (Some (inr n3)) t (n'2, jr'0, jtb'0)).
+ remember (jtree_table' n0 (Some (inr n3)) t (n2, jr''0, jtb0)).
+ destruct n4. destruct p.
+ destruct n5. destruct p.
+ apply IHlj with (n:=n0) (n':=n'0) (n1:=n5) (n'1:=n4) (jtb'1:=j) (jtb1:=j0)
+ (jr''1:=l1) (jr'1:=l0) in H6.
+ apply H6. rewrite clear_node_index_app.
+ replace l0 with (snd (fst (jtree_table' n'0 (Some (inr n3)) t (n'2, jr'0, jtb'0)))).
+ replace l1 with (snd (fst (jtree_table' n0 (Some (inr n3)) t (n2, jr''0, jtb0)))).
+ clear IHlj. apply H5. auto. rewrite <- Heqn5. auto.
+ rewrite <- Heqn4. auto.
+
+ simpl.
+ remember (S n') as n'1. remember (app jr' [ind_root_node m' n']) as jr'1.
+ remember (jtable_set jtb' m' n' k) as jtb'1.
+ remember (S n) as n1. remember (app jr'' [ind_root_node m n]) as jr''1.
+ remember (jtable_set jtb m n k) as jtb1. 
+ assert (clear_node_index (jr ++ jr'1) = clear_node_index jr''1).
+ subst. rewrite 3 clear_node_index_app. simpl. 
+ rewrite <- H0. rewrite clear_node_index_app. apply app_assoc.
+ generalize H1.
+ generalize jr'1.
+ generalize jr''1. generalize jtb1.
+ generalize jtb'1. generalize n'1. 
+ generalize n1. generalize n'. generalize n.
+ induction mj; intros. simpl.
+ rewrite <- clear_node_index_app. auto. simpl.
+ destruct a. replace (map snd ((k0, t) :: mj)) with
+ (t :: map snd mj) in H; auto. inversion H. clear H.
+ simpl. 
+ remember (jtree_table' n'0 (Some (inl k0)) t (n'2, jr'0, jtb'0)).
+ remember (jtree_table' n0 (Some (inl k0)) t (n2, jr''0, jtb0)).
+ destruct n3. destruct p.
+ destruct n4. destruct p.
+ apply IHmj with (n:=n0) (n':=n'0) (n1:=n4) (n'1:=n3) (jtb'1:=j)
+ (jtb1:=j0) (jr''1:=l1) (jr'1:=l0) in H6.
+ apply H6. rewrite clear_node_index_app.
+ replace l0 with (snd (fst (jtree_table' n'0 (Some (inl k0)) t (n'2, jr'0, jtb'0)))).
+ replace l1 with (snd (fst (jtree_table' n0 (Some (inl k0)) t (n2, jr''0, jtb0)))).
+ clear IHmj. apply H5. auto. rewrite <- Heqn4. auto.
+ rewrite <- Heqn3. auto.
+Qed.
+
+
+Lemma jtable_nodes_equal': forall jt m k n jr jtb, app (clear_node_index jr) (jtree_nodes jt) = 
+                                     clear_node_index (snd (fst (jtree_table' m k jt (n, jr, jtb)))).
+Proof.
+ intros jt.
+ induction jt using tree_ind'; intros.
+ simpl. rewrite clear_node_index_app. simpl. auto.
+
+ simpl.
+ remember (S n) as n1.
+ remember (jtable_set jtb m n k) as jtb1.
+ replace (clear_node_index jr ++
+ root_node :: flatten (map (compose jtree_nodes snd) lj))%list with
+ ((clear_node_index (jr ++ [ind_root_node m n]) ++ 
+  flatten (map (compose jtree_nodes snd) lj)))%list.
+ remember (app jr  [ind_root_node m n]) as jr1.
+ generalize n1 jr1 jtb1 n. 
+ induction lj; intros.
+ simpl. apply app_nil_r. 
+ destruct a.
+ replace (map snd ((n3, t) :: lj)) with (t::map snd lj) in H; auto.
+ inversion_clear H. simpl.
+ remember (jtree_table' n2 (Some (inr n3)) t (n0, jr0, jtb0)).
+ destruct n4. destruct p.
+ replace (clear_node_index jr0 ++
+  compose jtree_nodes snd (n3, t) ++
+    flatten (map (compose jtree_nodes snd) lj))%list with 
+ ((clear_node_index jr0 ++ jtree_nodes t) ++
+    flatten (map (compose jtree_nodes snd) lj))%list.
+ rewrite <- IHlj with (jr1:=l).
+ rewrite H0 with (m:=n2) (k:=Some (inr n3)) (n:=n0) (jtb:=jtb0).
+ replace l with (snd (fst (jtree_table' n2 (Some (inr n3)) t (n0, jr0, jtb0)))).
+ auto. rewrite <- Heqn4. auto. auto. rewrite app_assoc.
+ unfold compose. simpl. auto. rewrite clear_node_index_app.
+ simpl. rewrite <- app_assoc. simpl. auto.
+
+ simpl.
+ remember (S n) as n1.
+ remember (jtable_set jtb m n k) as jtb1.
+ replace (clear_node_index jr ++
+ root_node :: flatten (map (compose jtree_nodes snd) mj))%list with
+ ((clear_node_index (jr ++ [ind_root_node m n]) ++ 
+  flatten (map (compose jtree_nodes snd) mj)))%list.
+ remember (app jr  [ind_root_node m n]) as jr1.
+ generalize n1 jr1 jtb1 n. 
+ induction mj; intros.
+ simpl. apply app_nil_r. 
+ destruct a.
+ replace (map snd ((k0, t) :: mj)) with (t::map snd mj) in H; auto.
+ inversion_clear H. simpl.
+ remember (jtree_table' n2 (Some (inl k0)) t (n0, jr0, jtb0)).
+ destruct n3. destruct p.
+ replace (clear_node_index jr0 ++
+  compose jtree_nodes snd (k0, t) ++
+    flatten (map (compose jtree_nodes snd) mj))%list with 
+ ((clear_node_index jr0 ++ jtree_nodes t) ++
+    flatten (map (compose jtree_nodes snd) mj))%list.
+ rewrite <- IHmj with (jr1:=l).
+ rewrite H0 with (m:=n2) (k:=Some (inl k0)) (n:=n0) (jtb:=jtb0).
+ replace l with (snd (fst (jtree_table' n2 (Some (inl k0)) t (n0, jr0, jtb0)))).
+ auto. rewrite <- Heqn3. auto. auto. rewrite app_assoc.
+ unfold compose. simpl. auto. rewrite clear_node_index_app.
+ simpl. rewrite <- app_assoc. simpl. auto.
+Qed.
+
+
+Lemma jtable_nodes_equal: forall jt, jtree_nodes jt = 
+                                     clear_node_index (fst (jtree_table jt)).
+Proof.
+ intros. unfold jtree_table. simpl. rewrite <- jtable_nodes_equal'.
+ simpl. auto.
+Qed.
+
+Fixpoint jtable_tree' (n: nat) (m: nat) 
+                      (jr: jtable_row) (jtb: jtable) {struct n}: option jtree :=
+match n with
+| O => None
+| S n' => 
+let mr := nth_error jtb m in
+match mr with
+| Some r => let r' := indexate r in 
+            let fix iter_row r jt :=
+            match r with
+            | [] => jt
+            | (_, None)::rs => iter_row rs jt
+            | (n, Some (inr k))::rs => 
+                                   let md := nth_error jr n in
+                                   iter_row rs match md with
+                                   | Some (data_node s) => 
+                                               match jt with
+                                               | None => Some (tlbranch [(k, tleaf s)])
+                                               | Some (tlbranch tl) => Some (tlbranch (app tl [(k, tleaf s)]))
+                                               | _ => jt
+                                               end
+                                   | Some root_node => let mt' := jtable_tree' n' n jr jtb in
+                                               match mt' with
+                                               | None => jt
+                                               | Some t' => 
+                                                 match jt with
+                                                 | None => Some (tlbranch [(k, t')])
+                                                 | Some (tlbranch tl) => Some (tlbranch (app tl [(k, t')]))
+                                                 | _ => jt
+                                                 end
+                                               end
+                                   | None => None
+                                   end
+            | (n, Some (inl k))::rs => 
+                                   let md := nth_error jr n in
+                                   iter_row rs match md with
+                                   | Some (data_node s) => 
+                                               match jt with
+                                               | None => Some (tmbranch [(k, tleaf s)])
+                                               | Some (tmbranch tm) => Some (tmbranch (app tm [(k, tleaf s)]))
+                                               | _ => jt
+                                               end
+                                   | Some root_node => let mt' := jtable_tree' n' n jr jtb in
+                                               match mt' with
+                                               | None => jt
+                                               | Some t' => 
+                                                 match jt with
+                                                 | None => Some (tmbranch [(k, t')])
+                                                 | Some (tmbranch tm) => Some (tmbranch (app tm [(k, t')]))
+                                                 | _ => jt
+                                                 end
+                                               end
+                                   | None => None
+                                   end
+            end in
+            let mjt' := iter_row r' None in
+            match mjt' with
+            | None => Some (tlbranch [])
+            | _ => mjt' 
+            end
+| None => None
+end
+end.
+
+Definition jtable_tree jr jtb := jtable_tree' ((length jr)*(length jr)) 0 jr jtb.
+
+Fixpoint path_ind' (n:nat) (lk: jpath) (jr: list indjnode) (jtb: jtable) : 
+                                                  option (nat + nat*nat) :=
+match lk with
+| [] => let mv := nth_error jr n in
+        match mv with
+        | None => None
+        | Some (ind_data_node n _) => Some (inl n)
+        | Some (ind_root_node m n) => Some (inr (m, n))
+        end
+| k::ks => let mr := nth_error jtb n in
+           match mr with
+           | None => None
+           | Some r => let mn := find k r in
+                       match mn with
+                       | None => None
+                       | Some n => path_ind' n ks jr jtb
+                       end
+           end
+end.
+
+Definition tree_path_ind lk jt := let (jr, tb) := jtree_table jt in
+                                  path_ind' 0 lk jr tb.
+
+
+Definition table_json_default jr tb j :=
+let mtr := jtable_tree jr tb in
+match mtr with
+| None => j
+| Some tr => let mj' := tree_json  tr in
+                         match mj' with
+                         | None => j
+                         | Some j' => j'
+                         end
+end.
+
+Eval compute in (tree_path_ind [inr 2; inl "baz"; inl "x"]
+                 (json_tree ('[{"foo" # '[$"Andy"; $"Peter"]}; 
+                    {"bar" # $"Good"};
+                    {"baz" # {"x" # '[$"d"; $"f"]}}]))).
+                    
+Eval compute in (tree_path_ind [inr 1; inl "bar"]
+                 (json_tree ('[{"foo" # '[$"Andy"; $"Peter"]}; 
+                    {"bar" # $"Good"};
+                    {"baz" # {"x" # '[$"d"; $"f"]}}]))).
+
+                    
+Eval compute in  (nth_error (snd (jtree_table
+                 (json_tree ('[{"foo" # '[$"Andy"; $"Peter"]}; 
+                    {"bar" # $"Good"};
+                    {"baz" # {"x" # '[$"d"; $"f"]}}])))) 8).
+
+
+(*tests*)
+
+Let json1 := '[{"foo" # '[$"Andy"; $"Peter"]}; 
+                    {"bar" # $"Good"};
+                    {"baz" # {"x" # '[$"d"; $"f"]}}].
+Let jtree1 := json_tree json1.
+Let tn1 := jtree_nodes jtree1.
+Let jtb10 := jtable_fill (length tn1) None.
+Let jtb1 := jtree_table jtree1.
+Eval compute in jtb1.
+Let jtree1':= jtable_tree tn1 (snd jtb1).
+
+Example jtt_eq1: Some jtree1 = jtree1'.
+Proof. compute. auto. Qed.
+
+Example jtt_eq2: tn1 = clear_node_index (fst jtb1).
+Proof. auto. Qed.
+
