JsonTransformers.v
@@ -1,0 +1,353 @@
+Require Import String.
+Require Import Lists.List.
+Require Import Coq.Init.Nat.
+Require Import Coq.Program.Basics.
+
+Require Export Json.
+Require Export JsonTree.
+Require Export JsonTable.
+
+Import ListNotations.
+Import JsonNotations.
+
+Local Open Scope list_scope.
+Local Open Scope string_scope.
+Local Open Scope json_scope.
+
+Definition path_tree (ls: list string) root jt : list jpath :=
+let mt := tree_getin root jt in 
+match mt with 
+| None => []
+| Some jt => let jts := fold_right (fun s jts => let mts := map (tree_wild_get (from_string s)) jts in
+                                    let ts := flatten mts in
+                                    ts) [([],jt)] ls in
+                        map (fun p => app root (fst p)) jts
+end.
+
+Definition path_parse (s: string) (root: jpath) jt : list jpath :=
+let ls := split_string s "." in
+path_tree (rev ls) root jt.
+
+Definition do_at_nodes (j: json) (f: jpath -> json -> json) (path: string) : json :=
+let jt := json_tree j in
+let llk := path_parse path [] jt in
+fold_right f j llk. 
+
+Definition json_rename (newv: JsonData + key) (lk: jpath) (j: json) :=
+let tr := json_tree j in
+let (jr, tb) := jtree_table tr in
+let minds := tree_path_ind lk tr in
+match minds, newv with
+| None, _  => j
+| Some (inl k), inl newv => 
+                  let jr' := replace k (clear_node_index jr) (data_node newv) in
+                  table_json_default jr' tb j
+| Some (inl k), inr newv =>  let tb' := fold_right (fun m tb => let x := mnth_error tb m k in
+                                                                if x then jtable_set tb m k (Some (inl newv))
+                                                                     else tb) tb (seq 0 (length jr)) in
+                             table_json_default (clear_node_index jr) tb' j
+| Some (inr (m, n)), inr newv => 
+                  let tb' := jtable_set tb m n (Some (inl newv)) in
+                  table_json_default (clear_node_index jr) tb' j 
+| _, _ =>  j
+end.
+
+
+Inductive DestructStrategy := DestructStrategy0.
+
+Inductive IndMergeStrategy := 
+| IndRightMergeToNumber : IndMergeStrategy
+| IndRightMergeToKey : (key -> key) -> IndMergeStrategy.
+
+Fixpoint merge_inds (ilt ilf: list (option jpoint)) 
+                    (s:IndMergeStrategy) (b: bool):=
+match ilt, ilf with
+| [], ilf' => ilf'
+| ilt', [] => ilt'
+| None::ilt', (Some x)::ilf' => let l := merge_inds ilt' ilf' s b in
+                         match x, s with
+                         | inl kx, IndRightMergeToNumber => (Some (inr 0))::l
+                         | inr ix, IndRightMergeToNumber => (Some x)::l
+                         | inl kx, IndRightMergeToKey f => (Some (inl (f kx)))::l
+                         | inr ix, IndRightMergeToKey f => (Some (inl (f (writeNat ix))))::l
+                         end
+| x::ilt', None::ilf' => x::(merge_inds ilt' ilf' s b)
+(*shouldn't be happened*)
+| (Some x)::ilt',(Some y)::ilf' => 
+                            let z:= match x,y with
+                                    | inl kx, inl ky => inl (kx ++ "." ++ ky)
+                                    | inl kx, inr iy => inl (kx ++ "." ++ (indexNat iy))
+                                    | inr ix, inl ky => inr ix (*FIXME:will be ignored, but...*)
+                                    | inr ix, inr iy => inr ix (*FIXME:will be ignored, but...*)
+                                    end in
+                            if b then (Some x)::(merge_inds ilt' ilf' s b)
+                                 else (Some z)::(merge_inds ilt' ilf' s b)
+end.
+
+
+Definition json_destruct (lk: jpath) (j: json): json :=
+let tr := json_tree j in
+let (jr, tb) := jtree_table tr in
+let minds := tree_path_ind lk tr in
+match minds with
+| None => j
+| Some (inl k) => let tb' := fold_right (fun m tb => jtable_set tb m k None) 
+                                          tb (seq 0 (length jr)) in
+                  table_json_default (clear_node_index jr) tb' j 
+
+| Some (inr (m, n)) => let milt := nth_error tb m in
+                       let milf := nth_error tb n in
+                       let mtr := tree_getin (removelast lk) tr in
+                       let last := last lk (inl "") in
+                       let slast := match last with
+                                    | inr k => writeNat k
+                                    | inl k => k
+                                    end in
+                       match milt, milf, mtr with
+                           | None, _, _ => j
+                           | _, None, _ => j
+                           | _, _, None => j
+                           | _, _, Some (tleaf _) => j
+                           | Some ilt, Some ilf, Some (tlbranch _)  => 
+                                       let ilt' := merge_inds ilt ilf IndRightMergeToNumber true in
+                                       let tb' := replace m tb ilt' in
+                                       let tb'' := jtable_set tb' m n None in
+                                       table_json_default (clear_node_index jr) tb'' j
+                           | Some ilt, Some ilf, Some (tmbranch _)  => 
+                                       let ilt' := merge_inds ilt ilf (IndRightMergeToKey (fun k => (append (append slast "-") k))) true in
+                                       let tb' := replace m tb ilt' in
+                                       let tb'' := jtable_set tb' m n None in
+                                       table_json_default (clear_node_index jr) tb'' j
+                       end
+end.
+
+Definition json_remove (lk: jpath) (j: json): json :=
+let tr := json_tree j in
+let (jr, tb) := jtree_table tr in
+let minds := tree_path_ind lk tr in
+match minds with
+| None => j
+| Some (inl k) => let tb' := fold_right (fun m tb => jtable_set tb m k None) 
+                                          tb (seq 0 (length jr)) in
+                  table_json_default (clear_node_index jr) tb' j 
+
+| Some (inr (m, n)) => let tb' := jtable_set tb m n None in
+                       table_json_default (clear_node_index jr) tb' j
+                           
+end.
+
+Definition json_modify (f: jtree -> jtree) (lk: jpath) (j: json) : json :=
+let tr := json_tree j in
+let tr' := tree_modify lk tr f in
+let mj' := tree_json tr' in
+match mj' with
+| None => j
+| Some j' => j'
+end.
+
+(*CREATE AT "*.telecom"*)
+Definition json_create (s: string) (lk: jpath) (j: json) : json :=
+let jt := json_tree j in
+let p := from_string s in
+let mjt' := tree_getin lk jt in
+let jt' := match mjt' with 
+| None => jt
+| Some jt' => let mjt'' := tree_get p jt' in
+              let pth := app lk [p] in
+              match mjt'' with
+              | Some _ => jt
+              | None => match p with
+                        | inr k => tree_mergein lk jt (tlbranch [(k, tlbranch [])]) MergeStrategy0
+                        | inl k => tree_mergein lk jt (tmbranch [(k, tlbranch [])]) MergeStrategy0
+                        end
+              end
+end in
+(*let jt' := fold_right (fun p (pjt: jpath*jtree) => let (pth, jt) := pjt in
+                                    let pth' := app pth [p] in
+                                    let mjt' := tree_getin pth' jt in
+                                    match mjt' with
+                                    | Some _ => (pth', jt)
+                                    | None => match p with
+                                              | inr k => (pth', tree_mergein pth jt (tlbranch [(k, tlbranch [])]) MergeStrategy0)
+                                              | inl k => (pth', tree_mergein pth jt (tmbranch [(k, tlbranch [])]) MergeStrategy0)
+                                              end
+                                    end) ([], jt) lk in*)
+let mj' := tree_json jt' in
+match mj' with
+| None => j
+| Some j' => j'
+end.
+
+(* COLLECT "telecom*" TO "telecom" AT "*" *)
+Definition json_collect (what pto: string) f (root: jpath) (j: json) : json :=
+let jt := json_tree j in
+let llkf := path_parse what root jt in
+let llkt := path_parse pto root jt in
+let jt' := fold_left (fun jt lkf => 
+                        fold_right (fun lkt jt => tree_submerge_with lkt lkf f jt MergeStrategy0) jt llkt) llkf jt in
+let mj' := tree_json jt' in
+match mj' with
+| None => j
+| Some j' => j'
+end.
+
+Definition json_zip_at (ks: list string) (root: jpath) (j: json) :=
+let jt := json_tree j in
+let llkf := flatten (map (fun s => path_parse s root jt) ks) in
+let trees := filterSome (map (fun p => tree_getin p jt) llkf) in 
+let jt' := tree_setin root jt (tlbranch (indexate (fold_left ziptrees' trees []))) in
+let mj' := tree_json jt' in
+match mj' with
+| None => j
+| Some j' => j'
+end.
+
+(*tests*)
+
+Example rename1: (json_rename (inr "y") [inr 2; inl "baz"; inl "x"]
+                  '[{"foo" # '[$"Andy"; $"Peter"]}; 
+                    {"bar" # $"Good"};
+                    {"baz" # {"x" # '[$"d"; $"f"]}}]    = 
+                   '[{"foo" # '[$"Andy"; $"Peter"]}; 
+                    {"bar" # $"Good"};
+                    {"baz" # {"y" # '[$"d"; $"f"]}}]).
+Proof. auto. Qed.
+
+Example rename2: (json_rename (inl "Mike") [inr 0; inl "foo"; inr 0]
+                  '[{"foo" # '[$"Andy"; $"Peter"]}; 
+                    {"bar" # $"Good"};
+                    {"baz" # {"x" # '[$"d"; $"f"]}}] = 
+                   '[{"foo" # '[$"Mike"; $"Peter"]}; 
+                    {"bar" # $"Good"};
+                    {"baz" # {"x" # '[$"d"; $"f"]}}]).
+Proof. auto. Qed.
+
+Example rename3: json_rename (inr "y") [inr 1; inl "bar"]
+                  '[{"foo" # '[$"Andy"; $"Peter"]}; 
+                    {"bar" # $"Good"};
+                    {"baz" # {"x" # '[$"d"; $"f"]}}] = 
+                    '[{"foo" # '[$"Andy"; $"Peter"]}; 
+                    {"y" # $"Good"};
+                    {"baz" # {"x" # '[$"d"; $"f"]}}].
+Proof. auto. Qed.
+
+Let json2 := '[{"type" # $"person",
+                "name" # '[{"given" # '[$"Andy"; $"Michael"], "family" # $"Watson"};
+                            {"given" # '[$"Andrey"], "family" # $"Watsonov"}],
+                "telecom" # '[{"system" # $"phone", "value" # $"1234"};
+                              {"system" # $"phone", "value" # $"5678"};
+                              {"system" # $"mail", "value" # $"andy@watson.me"};
+                              {"system" # $"mail", "value" # $"andrey@mail.ru"}]
+                 };
+                {"type" # $"person",
+                "name" # '[{"given" # '[$"John"; $"Israel"], "family" # $"Koen"};
+                            {"given" # '[$"Ivan"], "family" # $"Koinov"}],
+                "telecom" # '[{"system" # $"phone", "value" # $"4321"};
+                              {"system" # $"phone", "value" # $"8765"};
+                              {"system" # $"mail", "value" # $"john@koen.me"}]
+                }].
+
+Let json3 := '[{"given1" # $"Andy Michael", "family1" # $"Watson",
+                "given2" # $"Andrey", "family2" #  $"Watsonov",
+                "phone1" # $"1234", "phone2" # $"5678",
+                "mail1" # $"andy@watson.me",
+                "mail2" # $"andrey@mail.ru"};
+                {"given1" # $"John Israel", "family1" # $"Koen",
+                "given2" # $"Ivan", "family2" #  $"Koinov",
+                "phone1" # $"4321", "phone2" # $"8765",
+                "mail1" # $"john@koen.me"}].
+
+Let tree2 := json_tree json2.
+Let tb22 := jtree_table tree2.
+Let tab2 := snd tb22.
+
+
+
+Eval compute in (path_parse "*.name" [] tree2).
+
+Let json21' := do_at_nodes json2 json_destruct "*.name".
+Eval compute in json21'.
+Eval compute in (json_getin [inr 0; inl "name-0"] json21').
+Eval compute in (json_getin [inr 0; inl "name-1"] json21').
+Let json22' := do_at_nodes json21' json_destruct "*.name*".
+Eval compute in json22'.
+Let json23' := do_at_nodes json22' (json_modify (concat_tree_with " ")) "*.name*given".
+Eval compute in json23'.
+Let json24' := do_at_nodes json23' json_destruct "*.telecom".
+Eval compute in json24'.
+Let json25' := do_at_nodes json24' (json_modify (fun t => let mt1 := tree_getin [inl "system"] t in
+                                                             let mt2 := tree_getin [inl "value"] t in
+                                                             match mt1, mt2 with
+                                                             | Some (tleaf s1), Some (tleaf s2) => 
+                                                                    (tmbranch [(s1, tleaf s2)])
+                                                             | _, _ => t
+                                                             end))  "*.telecom*".
+Eval compute in json25'.
+Let json26' := do_at_nodes json25' json_destruct "*.telecom*".
+Eval compute in json26'.
+Let json27' := do_at_nodes json26' (json_rename (inr "given1")) "*.name-0-given".
+Let json28' := do_at_nodes json27' (json_rename (inr "given2")) "*.name-1-given".
+Let json29' := do_at_nodes json28' (json_rename (inr "family1")) "*.name-0-family".
+Let json210' := do_at_nodes json29' (json_rename (inr "family2")) "*.name-1-family".
+Let json211' := do_at_nodes json210' (json_rename (inr "phone1")) "*.telecom-0-phone".
+Let json212' := do_at_nodes json211' (json_rename (inr "phone2")) "*.telecom-1-phone".
+Let json213' := do_at_nodes json212' (json_rename (inr "mail1")) "*.telecom-2-mail".
+Let json214' := do_at_nodes json213' (json_rename (inr "mail2")) "*.telecom-3-mail".
+Let json215' := do_at_nodes json214' json_destruct "*.type".
+
+Example mapping1 : json3 = json215'.
+Proof. compute. auto. Qed.
+
+Let json31' := do_at_nodes json3 (json_create "type") "*".
+Let json32' := do_at_nodes json31' (json_modify (fun _ => tleaf "person")) "*.type".
+Eval compute in json32'.
+
+Let json33' := do_at_nodes json32' (json_rename (inr "name-0-given")) "*.given1".
+Let json34' := do_at_nodes json33' (json_rename (inr "name-1-given")) "*.given2".
+Let json35' := do_at_nodes json34' (json_rename (inr "name-0-family")) "*.family1".
+Let json36' := do_at_nodes json35' (json_rename (inr "name-1-family")) "*.family2".
+Let json37' := do_at_nodes json36' (json_rename (inr "telecom-0-phone")) "*.phone1".
+Let json38' := do_at_nodes json37' (json_rename (inr "telecom-1-phone")) "*.phone2".
+Let json39' := do_at_nodes json38' (json_rename (inr "telecom-2-mail")) "*.mail1".
+Let json310' := do_at_nodes json39' (json_rename (inr "telecom-3-mail")) "*.mail2".
+
+Let json311' := do_at_nodes json310' (json_modify (split_tree_with " ")) "*.name*given".
+Eval compute in json311'.
+Let json312' := do_at_nodes json311' (json_create "'name-given") "*".
+Let json313' := do_at_nodes json312' (json_collect "name*given" "'name-given" (fun lk jt => tlbranch [(0, jt)])) "*".
+Eval compute in json313'.
+Let json314' := do_at_nodes json313' (json_create "'name-family") "*".
+Let json315' := do_at_nodes json314' (json_collect "name*family" "'name-family" (fun lk jt => tlbranch [(0, jt)])) "*".
+Eval compute in json315'.
+Let json316' := do_at_nodes json315' json_remove "*.name*".
+Eval compute in json316'.
+Let json317' := do_at_nodes json316' (json_create "name") "*".
+Let json318' := do_at_nodes json317' (json_collect "'name*" "name" (fun lk jt => let l := last lk (inl "error") in
+                                                                                 let sl := writeJPoint l in
+                                                                                 let sl' := split_string sl "-" in
+                                                                                 let sl'' := nth 1 sl' "error" in
+                                                                    tmbranch [(sl'', jt)])) "*".
+Eval compute in json318'.
+Let json319' := do_at_nodes json318' json_remove "*.'name*".
+Eval compute in json311'.
+Let json320' := do_at_nodes json319' (json_zip_at ["given"; "family"]) "*.name".
+Eval compute in json320'.
+Let json321' := do_at_nodes json320' (json_modify (map_tree_with ["given"; "family"])) "*.name".
+Eval compute in json321'.
+
+Let json322' := do_at_nodes json321' (json_create "'telecom") "*".
+Let json323' := do_at_nodes json322' (json_collect "telecom*" "'telecom" (fun lk jt => let l := last lk (inl "error") in
+                                                                                      let sl := writeJPoint l in
+                                                                                      let sl' := split_string sl "-" in
+                                                                                      let sl'' := last sl' "error" in
+                                                                        tlbranch [(0, tmbranch [("system", tleaf sl''); 
+                                                                                  ("value", jt)])])) "*".
+Eval compute in json323'.
+Let json324' := do_at_nodes json323' json_remove "*.telecom*".
+Eval compute in json324'.
+Let json325' := do_at_nodes json324' (json_rename (inr "telecom")) "*.'telecom".
+Eval compute in json325'.
+
+Example mapping2 : json2 = 
+                   json325'.
+Proof. compute. auto. Qed.
