JsonTree.v
@@ -1,0 +1,500 @@
+Require Import String.
+Require Import Lists.List.
+Require Import Coq.Init.Nat.
+Require Import Coq.Program.Basics.
+
+Require Export Json. 
+Require Export CommonHelpers.
+Require Export StringHelpers.
+
+Import ListNotations.
+Import JsonNotations.
+
+Local Open Scope list_scope.
+Local Open Scope string_scope.
+Local Open Scope json_scope.
+
+Inductive tree (X Y: Set) : Set :=
+| tleaf : X -> @tree X Y
+| tlbranch : list (nat*tree X Y) -> tree X Y
+| tmbranch : list (Y*tree X Y) -> tree X Y.
+(*the empty tree can be written as "tlbranch []"*)
+
+Arguments tleaf [X] [Y].
+Arguments tlbranch [X] [Y].
+Arguments tmbranch [X] [Y].
+
+Section tree_ind'.
+
+Variable X Y: Set.
+Variable P: tree X Y -> Prop.
+
+Hypothesis tree_leaf_case : forall (x : X),
+    P (tleaf x).
+
+Hypothesis tree_list_case : forall (lj : list (nat*tree X Y)),
+    Forall P (map snd lj) -> P (tlbranch lj).
+
+Hypothesis tree_map_case : forall (mj : list (Y*tree X Y)),
+    Forall P (map snd mj) -> P (tmbranch mj).
+
+Fixpoint tree_ind' (t : tree X Y) : P t :=
+match t return (P t) with
+| tleaf x => tree_leaf_case x
+| tlbranch lt => tree_list_case lt
+        ((fix tree_list_ind (lt : list (nat*tree X Y)) : Forall P (map snd lt) :=
+          match lt with
+            | [] => Forall_nil P
+            | (k,t)::ltx => @Forall_cons (tree X Y) P t (map snd ltx) (tree_ind' t) (tree_list_ind ltx)
+          end) lt)
+| tmbranch lt => tree_map_case lt
+        ((fix tree_list_ind (lt : list (Y*tree X Y)) : Forall P (map snd lt) :=
+          match lt with
+            | [] => Forall_nil P
+            | (k,t)::ltx => @Forall_cons (tree X Y) P t (map snd ltx) (tree_ind' t) (tree_list_ind ltx)
+          end) lt)
+end.
+
+End tree_ind'.
+
+Definition jtree := tree JsonData key.
+
+Fixpoint json_tree (j: json): jtree :=
+match j with
+| $s => tleaf s
+| 'l => tlbranch (indexate (map json_tree l))
+| &m => let fix map_tree (mm: @key_map json) :=
+            match mm with
+            | empty => []
+            | mapkv k v kvs => (k, json_tree v)::map_tree kvs 
+            end in
+        tmbranch (map_tree m)
+end.
+
+Fixpoint tree_json (jt: jtree): option json :=
+match jt with
+| tleaf s => Some $s
+| tlbranch lt => let l := fold_right (fun (kt:nat*jtree) l =>
+                                    match l with
+                                    | Some l => let mj := tree_json (snd kt) in
+                                                       match mj with
+                                                       | Some j => Some (cons j l)
+                                                       | None => None
+                                                       end
+                                    | _ => None
+                                    end) (Some []) lt in
+                           match l with
+                           | None => None
+                           | Some l => Some 'l
+                           end
+| tmbranch mt => let m := fold_right (fun (kt: key*jtree) m =>  
+                                        let (k, t) := kt in
+                                        match k, m with 
+                                        | k, Some m => let mj := tree_json t in
+                                                           match mj with
+                                                           | Some j => Some (mapkv k j m)
+                                                           | None => None
+                                                           end
+                                        | _, _ => None 
+                                        end) (Some empty) mt in
+                                  match m with
+                                  | None => None
+                                  | Some m => Some &m
+                                  end
+end.
+
+Check json_ind'.
+
+Lemma tree_json_ind_ign: forall lj m n, fold_right
+  (fun (kt : nat * jtree) (l : option (list json)) =>
+   match l with
+   | Some l0 =>
+       match tree_json (snd kt) with
+       | Some j => Some (j :: l0)
+       | None => None
+       end
+   | None => None
+   end) (Some []) (indexate_with' m id (map json_tree lj)) =
+fold_right
+  (fun (kt : nat * jtree) (l : option (list json)) =>
+   match l with
+   | Some l0 =>
+       match tree_json (snd kt) with
+       | Some j => Some (j :: l0)
+       | None => None
+       end
+   | None => None
+   end) (Some []) (indexate_with' n id (map json_tree lj)).
+Proof.
+ intros lj. induction lj; intros. auto.
+ simpl. rewrite IHlj with (n:= S n).
+ auto.
+Qed.
+
+Lemma tree_json_inv: forall j, tree_json (json_tree j) = Some j.
+Proof.
+ intros. induction j using json_ind'.
+ simpl. auto.
+ induction lj. auto.
+ inversion_clear H. apply IHlj in H1.
+ simpl. rewrite H0. simpl in H1.
+ remember (fold_right
+         (fun (kt : nat * jtree) (l : option (list json)) =>
+          match l with
+          | Some l0 =>
+              match tree_json (snd kt) with
+              | Some j => Some (j :: l0)
+              | None => None
+              end
+          | None => None
+          end) (Some []) (indexate (map json_tree lj))).
+ replace (fold_right
+      (fun (kt : nat * jtree) (l : option (list json)) =>
+       match l with
+       | Some l0 =>
+           match tree_json (snd kt) with
+           | Some j => Some (j :: l0)
+           | None => None
+           end
+       | None => None
+       end) (Some []) (indexate_with' 1 id (map json_tree lj))) with o.
+ destruct o; inversion H1; auto. rewrite Heqo.
+ unfold indexate.
+ apply tree_json_ind_ign. 
+ induction mj. auto.
+ inversion_clear H. apply IHmj in H1.
+ simpl. rewrite H0. simpl in H1.
+ remember (fold_right
+         (fun (kt : key * jtree) (m : option key_map) =>
+          let (k, t) := kt in
+          match m with
+          | Some m0 => match tree_json t with
+                       | Some j => Some ((k) # (j) m0)
+                       | None => None
+                       end
+          | None => None
+          end) (Some empty)
+         ((fix map_tree (mm : key_map) : list (key * jtree) :=
+             match mm with
+             | empty => []
+             | (k) # (v) kvs => (k, json_tree v) :: map_tree kvs
+             end) mj)).
+ destruct o; inversion H1; auto. 
+Qed. 
+
+Inductive MergeStrategyIn := SMergeRight | SReplace | SMergeLeft | SExchange. 
+Inductive MergeStrategyOut := SRemoveOrigin | SLeaveOrigin.
+Inductive NameStrategy := 
+| SRenameNode: key -> NameStrategy
+| SLeaveNodeName: NameStrategy.
+
+Inductive MergeStrategyT := 
+| MergeStrategy: MergeStrategyIn -> MergeStrategyOut ->
+                 NameStrategy -> NameStrategy -> MergeStrategyT.
+
+Definition MergeStrategy0 := MergeStrategy SMergeRight SLeaveOrigin 
+                             SLeaveNodeName SLeaveNodeName.
+
+Definition merge_trees (t1 t2: jtree) (s: MergeStrategyT) : jtree :=
+match t1,t2 with
+| tleaf s1, tleaf s2 => tlbranch (indexate [t1; t2])
+
+| tleaf s1, tlbranch tl2 => tlbranch (indexate (t1::(map snd tl2)))
+| tlbranch tl1, tleaf s2 => tlbranch (indexate (app (map snd tl1) [t2]))
+| tlbranch tl1, tlbranch tl2 => tlbranch (indexate (app (map snd tl1) (map snd tl2)))
+
+| tleaf s1, tmbranch tm2 => tmbranch ((indexNat 0, t1)::tm2)
+| tmbranch tm1, tleaf s2 =>  tmbranch (app tm1 [(indexNat 0, t2)])
+| tmbranch tm1, tmbranch tm2 => tmbranch (app tm1 tm2)
+
+| tlbranch tl1, tmbranch tm2 => tmbranch (app (indexate_with indexNat (map snd tl1)) tm2)
+| tmbranch tm1, tlbranch tl2 => tmbranch (app tm1 (indexate_with indexNat (map snd tl2)))
+end.
+
+
+Definition tlookup {X} (tm: list (key*(tree X key))) (k: key) :=
+firstSome (map (fun (k'v: key*(tree X key)) => let (k', v) := k'v in
+                           if (string_dec k k') then Some v else None) tm).
+
+Definition tlookup_ind {X} (tm: list (key*(tree X key))) (k: key) :=
+firstSome_ind (map (fun (k'v: key*(tree X key)) => let (k', v) := k'v in
+                           if (string_dec k k') then Some v else None) tm).
+
+Fixpoint tree_get (kk: jpoint) (jt: jtree) {struct jt}: option (nat*jtree) :=
+match kk with
+| inl k => match jt with
+              | tmbranch tm => tlookup_ind tm k
+              | _ => None
+           end
+| inr k => match jt with
+              | tlbranch tl  => nth_error tl k
+              | _ => None
+           end
+end.
+
+Fixpoint tree_getin (lk: jpath) (jt: jtree): option jtree :=
+match lk with
+| [] => Some jt
+| k::ks => let mjt' := tree_get k jt in
+           match mjt' with
+           | None => None
+           | Some (_,jt') => tree_getin ks jt'
+           end 
+end.
+
+Fixpoint tree_setin (lk: jpath) (to_jt jt: jtree): jtree :=
+match lk with
+| [] => jt
+| k::ks => let mjt' := tree_get k to_jt in
+           match mjt' with
+           | None => to_jt
+           | Some (n, to_jt') => let nt := tree_setin ks to_jt' jt in
+                                 match k, to_jt with
+                                 | inr k, tlbranch tl => (tlbranch (replace n tl (k, nt)))
+                                 | inl k, tmbranch tm => (tmbranch (replace n tm (k, nt)))
+                                 | _,_ => to_jt
+                                 end
+           end 
+end.
+
+Definition tree_mergein (lk: jpath) (to_jt jt: jtree) s: jtree :=
+let mjt':= tree_getin lk to_jt in
+match mjt' with
+| None => to_jt
+| Some to_jt' => tree_setin lk to_jt (merge_trees to_jt' jt s)
+end.
+
+Definition tree_submerge_with (lk_to lk_from: jpath) 
+                              (f: jpath -> jtree -> jtree) (jt: jtree) (s: MergeStrategyT): jtree :=
+let mjt_from' := tree_getin lk_from jt in
+match mjt_from' with
+| Some jt_from' => tree_mergein lk_to jt (f lk_from jt_from') s
+| None => jt
+end.
+
+Definition tree_submerge (lk_to lk_from: jpath) 
+                         (jt: jtree) (s: MergeStrategyT): jtree :=
+tree_submerge_with lk_to lk_from (fun _ jt => jt) jt s.
+
+Definition tree_modify (lk_in: jpath) (jt: jtree) (f: jtree -> jtree) : jtree :=
+let mjt' := tree_getin lk_in jt in
+match mjt' with
+| Some jt' => tree_setin lk_in jt (f jt')
+| None => jt
+end.
+
+Definition concat_tree_with (d: JsonData) (jt: jtree): jtree :=
+match jt with
+| tleaf s => tleaf s
+| tlbranch tl => tleaf (fold_right (fun i r => match i with
+                                        | (_, tleaf s) => if (string_dec r "") then s 
+                                                          else (s ++ d ++ r)
+                                        | _ => r
+                                        end) ""  tl)
+| tmbranch tm => tleaf (fold_right (fun i r => match i with
+                                        | (_, tleaf s) => if (string_dec r "") then s 
+                                                          else (s ++ d ++ r)
+                                        | _ => r
+                                        end) ""  tm)
+end.
+
+Inductive jnode := 
+| data_node: JsonData -> jnode
+| root_node: jnode.
+
+Definition jtable_row := list jnode.
+
+Fixpoint json_nodes (j: json): jtable_row :=
+match j with
+| $s => [data_node s]
+| 'l => root_node::flatten (map json_nodes l)
+| &m => let fix map_nodes (mm: @key_map json): jtable_row :=
+            match mm with
+            | empty => []
+            | mapkv k v kvs => app (json_nodes v) (map_nodes kvs)
+            end in
+        root_node::map_nodes m
+end.
+
+Fixpoint jtree_nodes (jt: jtree): jtable_row :=
+match jt with
+| tleaf s => [data_node s]
+| tlbranch tl => root_node::flatten (map (compose jtree_nodes snd) tl)
+| tmbranch tm => root_node::flatten (map (compose jtree_nodes snd) tm)
+end.
+
+Lemma jtree_nodes_ind_ign: forall X Y T (f:Y->T) m n ind1 ind2 l,
+            map (fun xy : X * Y => f (snd xy)) (indexate_with' m ind1 l) = 
+            map (fun xy : X * Y => f (snd xy)) (indexate_with' n ind2 l).
+Proof.
+ intros. generalize dependent m. generalize dependent n. 
+ induction l; intros; auto. simpl. rewrite IHl with (n:= S n).
+ auto.
+Qed.
+
+
+Lemma jtree_nodes_equal: forall j, json_nodes j = jtree_nodes (json_tree j).
+Proof.
+ intros. induction j using json_ind'.
+ simpl. auto. induction lj. simpl. auto.
+ inversion_clear H. apply IHlj in H1. 
+ simpl. unfold compose. simpl. rewrite <- H0.
+ simpl in H1. inversion H1. clear H1.
+ rewrite H2. unfold compose. unfold indexate.
+ rewrite jtree_nodes_ind_ign with (n:=1) (ind2:=id). auto.
+ induction mj. simpl. auto.
+ inversion_clear H. apply IHmj in H1. 
+ simpl. unfold compose. simpl. rewrite <- H0.
+ simpl in H1. inversion H1. clear H1.
+ rewrite H2. unfold compose. auto.
+Qed.
+
+
+Definition split_tree_with (d: JsonData) (jt: jtree): jtree :=
+match jt with
+| tleaf s => let ss := split_string s d in
+             tlbranch (indexate (map (@tleaf JsonData key) ss))
+| _ => jt (* FIXME *)
+end.
+
+Definition tree_wild_get (p: jpoint) (jpt: jpath*jtree): list (jpath*jtree) :=
+let (p0, jt) := jpt in
+match p with
+| inr k => let mt := tree_get p jt in
+           match mt with
+           | None => []
+           | Some (_, t) => [(app p0 [p], t)]
+           end
+| inl k => match jt with
+           | tleaf s => []
+           | tlbranch tl => map (fun kt => (app p0 [inr (fst kt)], snd kt))
+                            (filter (fun (kt:nat*jtree) => let (k', t) := kt in
+                                     match_string k (indexNat k')) tl)
+           | tmbranch tm => map (fun kt => (app p0 [inl (fst kt)], snd kt))
+                            (filter (fun (kt:key*jtree) => let (k', t) := kt in
+                                     match_string k k') tm)
+           end
+end.
+
+Definition zip_tree_with (ks: list key) (jt: jtree) : jtree :=
+match jt with
+| tleaf _ => jt
+| tlbranch tl => tmbranch (zip_first_with ks tl (tlbranch []) indexNat)
+| tmbranch tm => tmbranch (zip_first_with ks tm (tlbranch []) (@id key))
+end.
+
+Definition map_tree_with (ks: list key) (jt: jtree) : jtree :=
+match jt with
+| tleaf _ => jt
+| tlbranch tl => tlbranch (map (fun (kt:nat*jtree) => let (k,t) := kt in  
+                                          (k, zip_tree_with ks t)) tl)
+| tmbranch tm => tmbranch (map (fun (kt:key*jtree) => let (k,t) := kt in  
+                                          (k, zip_tree_with ks t)) tm)
+end.
+
+Definition map_tree_with_old (ks: list key) (jt: jtree) : jtree :=
+match jt with
+| tleaf _ => jt
+| tlbranch tl => tlbranch (indexate (map (fun (ks:nat*key) => let (k,s):=ks in 
+                                let txs := filterSome (map (tree_get (inr k)) (map snd tl)) in
+                                tmbranch [(s, tlbranch txs)] ) (indexate ks)))
+| _ => jt
+end.
+
+Fixpoint ziptrees' (ll : list jtree)  (l: jtree) :=
+match ll, l with
+| _, tlbranch [] => ll
+| [], tlbranch ((_::_) as l) => map (fun x => tlbranch [x]) l
+| (tlbranch lx)::lxs, tlbranch (x::xs) => (tlbranch (app lx [x]))::(ziptrees' lxs (tlbranch xs))
+| _,_ => ll
+end.
+
+(*tests*)
+
+Let json1 := '[{"foo" # '[$"Andy"; $"Peter"]}; 
+                    {"bar" # $"Good"};
+                    {"baz" # {"x" # '[$"d"; $"f"]}}].
+Let jtree1 := json_tree json1.
+
+Example tree_json1 : tree_json jtree1 = Some json1.
+Proof. auto. Qed.
+
+Example tree_setin1 : tree_json 
+                  (tree_setin [inr 2; inl "baz"; inl "x"; inr 1] jtree1 (tleaf "e")) = 
+                  Some '[{"foo" # '[$"Andy"; $"Peter"]}; 
+                    {"bar" # $"Good"};
+                    {"baz" # {"x" # '[$"d"; $"e"]}}].
+Proof. auto. Qed.
+
+
+Example json_tree1 : jtree1 =
+        tlbranch [(0,
+          tmbranch
+            [("foo",
+             tlbranch
+               [(0, tleaf "Andy"); (1, tleaf "Peter")])]);
+         (1, tmbranch [("bar", tleaf "Good")]);
+         (2,
+         tmbranch
+           [("baz",
+            tmbranch
+              [("x",
+               tlbranch [(0, tleaf "d"); (1, tleaf "f")])])])].
+Proof. auto. Qed.
+
+Example tree_modify1: tree_json (tree_modify [inr 0; inl "foo"] jtree1 (concat_tree_with " ")) = 
+                  Some '[{"foo" # $"Andy Peter"}; 
+                    {"bar" # $"Good"};
+                    {"baz" # {"x" # '[$"d"; $"f"]}}].
+Proof. auto. Qed.
+
+Example tree_setin2: tree_json (tree_setin [inr 2; inl "baz"; inl "x"; inr 0] jtree1 (tleaf "e")) =
+                 Some '[{"foo" # '[$"Andy"; $"Peter"]}; 
+                    {"bar" # $"Good"};
+                    {"baz" # {"x" # '[$"e"; $"f"]}}].
+Proof. auto. Qed.
+
+Example tree_mergein1: tree_json (tree_mergein [inr 2; inl "baz"; inl "x"] jtree1 (tleaf "j") MergeStrategy0) =
+                    Some '[{"foo" # '[$"Andy"; $"Peter"]}; 
+                    {"bar" # $"Good"};
+                    {"baz" # {"x" # '[$"d"; $"f"; $"j"]}}].
+Proof. auto. Qed.
+
+Example tree_submerge1: tree_json (tree_submerge [inr 0] [inr 2; inl "baz"; inl "x"] jtree1 MergeStrategy0) = 
+                   Some '[{"foo" # '[$"Andy"; $"Peter"], "#0" # $"d", "#1" # $"f"}; 
+                    {"bar" # $"Good"};
+                    {"baz" # {"x" # '[$"d"; $"f"]}}].
+Proof. compute. auto. Qed.
+
+Let json2 := {"menu" # {"header" # $"SVG Viewer",
+    "items" # '[
+        {"id"# $"Open"};
+        {"id"# $"OpenNew", "label"# $"Open New"};
+        {"id"# $"ZoomIn", "label"# $"Zoom In"};
+        {"id"# $"ZoomOut", "label"# $"Zoom Out"};
+        {"id"# $"OriginalView", "label"# $"Original View"};
+        {"id"# $"Quality"};
+        {"id"# $"Pause"};
+        {"id"# $"Mute"};
+        {"id"# $"Find", "label"# $"Find..."};
+        {"id"# $"FindAgain", "label"# $"Find Again"};
+        {"id"# $"Copy"};
+        {"id"# $"CopyAgain", "label"# $"Copy Again"};
+        {"id"# $"CopySVG", "label"# $"Copy SVG"};
+        {"id"# $"ViewSVG", "label"# $"View SVG"};
+        {"id"# $"ViewSource", "label"# $"View Source"};
+        {"id"# $"SaveAs", "label"# $"Save As"};
+        {"id"# $"Help"};
+        {"id"# $"About", "label"# $"About Adobe CVG Viewer..."}]}}.
+
+Let tree2 := json_tree json2.
+Let json2' := tree_json tree2.
+
+Example tree_json2: Some json2 = json2'.
+Proof. auto. Qed.
+
+Example json_nodes1: json_nodes json1 = 
+                     [root_node; root_node; root_node; data_node "Andy";
+       data_node "Peter"; root_node; data_node "Good"; root_node;
+       root_node; root_node; data_node "d"; data_node "f"].
+Proof. auto. Qed.
