KeyMaps.v
@@ -1,0 +1,65 @@
+Require Import String.
+Require Import Lists.List.
+Require Import Coq.Init.Nat.
+Require Import Coq.Program.Basics. 
+Require Import CommonHelpers.
+
+Import ListNotations.
+Local Open Scope list_scope.
+
+Module Type KeySig.
+Parameter key : Set.
+Parameter eqKey : key -> key -> bool.
+Axiom eqKey_refl : forall k1 k2, eqKey k1 k2 = true <-> k1 = k2.
+End KeySig.
+
+Module KeyMap (ks: KeySig).
+Import ks.
+
+Hint Resolve eqKey_refl.
+
+Inductive key_map {X:Set} := 
+| empty: key_map
+| mapkv: key -> X -> key_map -> key_map.
+
+Fixpoint mapmap {X:Set} {Y:Set} (f: X -> Y) (m: @key_map X) :=
+match m with
+| empty => empty
+| mapkv k v kvs => mapkv k (f v) (mapmap f kvs)
+end. 
+
+Fixpoint mapkeymap {X:Set} {Y:Set} (f: key -> X -> Y) (m: @key_map X) : list Y :=
+match m with
+| empty => []
+| mapkv k v kvs => (f k v) :: (mapkeymap f kvs)
+end.
+
+Fixpoint mapkeymap' {X:Set} {Y:Set} (f: X -> Y) (m: @key_map X) : list Y :=
+match m with
+| empty => []
+| mapkv k v kvs => (f v) :: (mapkeymap' f kvs)
+end. 
+
+Definition mapkeymap'' {X:Set} {Y:Set} (f: X -> Y) (m: @key_map X) : list Y:=
+mapkeymap (fun _ v => f v) m.
+
+Lemma mapkeymap''equal: forall (X Y:Set) (f: X -> Y) m,
+                 mapkeymap'' f m = mapkeymap' f m.
+Proof.
+ intros. unfold mapkeymap''.
+ induction m. simpl. auto.
+ simpl. rewrite IHm. auto.
+Qed.
+
+Fixpoint merge_maps {X:Set} (m1 m2: @key_map X) :=
+match m1 with
+| empty => m2
+| mapkv k v m1' => merge_maps m1' (mapkv k v m2)
+end.
+
+Definition valuelist {X:Set} := mapkeymap' (@id X).
+
+Definition mlookup {X:Set} (m: @key_map X) (k: key) :=
+    firstSome (mapkeymap (fun k' v => if (eqKey k k') then Some v else None) m).
+
+End KeyMap.
