KeySig.v
@@ -1,0 +1,5 @@
+Module Type KeySig.
+Parameter key : Set.
+Parameter eqKey : key -> key -> bool.
+Axiom eqKey_refl : forall k1 k2, eqKey k1 k2 = true <-> k1 = k2.
+End KeySig.
